#notes #phgn100 #physics
Names: Alec Malcangio, Wyatt Maney, Evan Majeski


$$y = - \frac{b}{a}x + b$$

$$y - b = \frac{-b}{a}x$$
$$\frac{y-b}{\frac{-b}{a}}=x$$
$$x = \frac{(y-b)(a)}{-b}$$


$$I = \frac{1}{3}mL^{2}$$



$$dm = \sigma dA$$
$$dA = x * dy$$
$$dA =  \frac{(y-b)(a)}{-b} * dy$$
$$dm = \sigma * dA$$
$$I = \frac{1}{3}(dm) L^{2}$$
$$ I = \frac{1}{3}( \sigma * \frac{(y-b)(a)}{-b})dy * \left(\frac{(y-b)(a)}{-b}\right)^{2} $$

---
$$\int_{0}^{b}I$$
$$\frac{1}{3}\sigma \int \left(\frac{(y-b)(a)}{(-b)}\right)^{3}dy$$



---
 All the work in this section is wrong, somehow. If you can figure it out, I would love to know.

$$\frac{1}{3}\sigma \int (u)^{3}du$$
$$du = dy$$
$$\frac{1}{3}\sigma  ~ \frac{u^{4}}{4}du$$
$$\frac{\sigma u^{4}}{12}$$

$$ \frac{\sigma}{12} * \left((y-b)\frac{a}{-b} \right)^{4} $$

$$ 0 - \frac{\sigma}{12}\left(\frac{(-b)a}{-b} \right)^{4}$$

$$- \frac{\sigma}{12}( a)^{4}$$

---
Back to correct work.
$$\frac{1}{3}\sigma \int \left(\frac{(y-b)(a)}{(-b)}\right)^{3}dy$$
$$\frac{1}{3}\sigma (\frac{a}{-b})^{3} \int_{0}^{b}(y-b)^3dy$$
$$\frac{1}{3}\sigma (\frac{a}{-b})^{3}\int _{0}^{b}u^{3}du$$
$$du = dy$$
$$\frac{1}{3}\sigma (\frac{a}{-b})^{3} \frac{u^{4}}{4}$$
$$\frac{1}{3}\sigma \frac{(\frac{a}{-b})^{3}(y-b)^{4}}{4}$$
$$\frac{\sigma}{12}( \frac{a}{-b})^{3}(y-b)^{4}$$
$$-\frac{\sigma}{12}(\frac{a}{-b})^{3}(-b)^{4}$$

