#notes #phgn100 #physics

We still would start with the equation
$$I = \int_{0}^{L} (\lambda dx)x^{2} $$
For our integral, but now, when changing lambda out, we can't just pull it out front, instead-

$$I = c \int _{0}^{L} x ~ dx ~ x^{2}$$
$$I = c \int _{0}^{L} x^{3}dx$$
$$I = c ( \frac{x^{4}}{4})$$
So then, integrating over the bounds, moment of inertia is just going to come out to be $$I = c( \frac{L^{4}}{4})$$
So we picked up another power of x or two, and otherwise the equation looks pretty similar.