#notes #math112 #math #calc

## previously on
- have some shenanigans like $\sqrt{a^{2}-x^{2}}$, we let $x=a\sin(\theta)$

## today
- some shenanigans like $\sqrt{x^{2}+a^{2}}$
- Let $x=a\tan(\theta)$
- $dx=a\sec^{2}(\theta)d\theta$

### example
$$I = \int \frac{dx}{(x^{2}+9)^{2}}$$
$$I = \frac{dx}{(\sqrt{x^{2}+9})^{4}}$$
$$x=3\tan\theta, \theta = \tan^{-1}(\frac{x}{3})$$
$$dx=3\sec^{2}(\theta)d\theta$$
$$\int \frac{3\sec^{2}(\theta) d\theta}{(9\tan^{2}(\theta)+9)^{2}}$$
Factor out a 9, get a +1

$$= \int \frac{3\sec^{2}(\theta)}{81\sec^{4}(\theta)}d\theta$$
$$\frac{1}{27}\int \frac{1}{\sec^{2}(\theta)}d\theta$$
$$I = \frac{1}{27}\int \cos^{2}(\theta)d\theta$$
pythagorean squared bullshit woo!
$$I = \frac{1}{27}\int \frac{1\cos(2\theta)}{2}$$
$$I= \frac{1}{54} (\theta + \frac{1}{2}\sin(2\theta))+C$$
$$I = \frac{1}{54}(\tan^{-1}(\frac{x}{3})+ \frac{1}{2}\sin(2\theta))+C$$
$$I = \frac{1}{54}(\tan^{-1}(\frac{x}{3})+ \frac{1}{2}2\sin\theta\cos\theta)+C$$
double angle bullshit WOO!
$$\frac{1}{54}(\tan ^{-1}(\frac{x}{3})+ \frac{1}{2}\frac{x}{\sqrt{x^{2}+9}}* \frac{3}{\sqrt{x^{2}+9}})+C$$
- this might be off by a factor of two. i don't really care.


------------------------

### more bullshit (case 3)
$$\sqrt{x^{2}-a^{2}}$$
$$\text{Let }x=a\sec\theta$$
$$\theta = \sec^{-1}( \frac{x}{a})$$
$$dx = a\sec(\theta)\tan(\theta)d\theta$$

$$I = \int \frac{x^{3}}{(x^{2}-9)}$$

$$\text{Let } x= 3\sec(\theta)$$
$$dx = 3\sec(\theta)\tan(\theta)d\theta$$

$$I = \int \frac{\sec^{3}(\theta)}{(9\sec^{2}(\theta)-9)^{\frac{3}{2}}}$$
$$I = \int \frac{(3\sec(\theta))^{3}}{9(\sec^2(\theta)-1)}dx$$
$$I = \int \frac{27\sec^{3}(\theta)*3\sec(\theta)\tan(\theta)}{27\tan^{3}(\theta)}d\theta$$
$$I = 3 \int \sec^{4}(\theta)\tan^{-2}(\theta)d\theta$$

$$I = 3 \int (\tan^{2}(\theta)+1)\tan^{-2}\sec^{2}(\theta)d\theta$$
$$u = \tan(\theta), du = \sec^{2}(\theta)d\theta$$
$$I = 3 \int(u^{2}+1)u^{-2}du$$
$$3(u-u^{-1})+C$$
$$3(\tan(\theta))-\cot(\theta)+C$$
$$3( \frac{\sqrt{x^{2}-9}}{3} - \frac{3}{\sqrt{x^{2}-9}})+C$$
$$\sqrt{x^{2}-9} - \frac{9}{\sqrt{x^{2}-9}}+C$$


---

$$\frac{5x-2}{x^{2}-x}$$
$$\frac{2}{x}+ \frac{3}{x-1}= \frac{5x-2}{x^{2}-x}$$
Start out with some rational $f(x)$, defined as $\frac{P(x)}{Q(x)}$ 

---

### Case 1 is the easiest. this is my thirty-fourth reason why.
- Proper rational function with linear factors
- Proper: Degree of $P(x)<Q(x)$ (largest power)
- Linear factor: $(x-a_{1})(x-a_{2})....$ blah blah blah 
- Ideally, we want to rewrite as $P\frac{P(x)}{Q(x)}$ as constant over factors

##### example
$$\frac{P(x)}{Q(x)} = \frac{3x-1}{x^{2}-1}$$
$$\frac{3x-1}{(x-1)(x+1)} = \frac{A}{x-1} + \frac{B}{x+1}$$
we're unfortunately gonna need a common denominator, assorted other fractions
$$\frac{3(x-1)}{(x-1)(x+1)}= \frac{A(x+1)+ B(x-1)}{(x-1)(x+1)}$$
$$3x-1= A(x+1)+B(x-1)$$
$$3x-1 = Ax+A +Bx-B$$
$$3x=Ax+Bx$$
$$3 =A+B$$
$$A=3-B$$
$$A-B = -1$$
$$3-B-B=-1, 3-2B=-1$$
$$-1 +2B=3$$
$$4=2B, B=2, A=1$$

$$\frac{(x+1)+2(x-1)}{(x-1)(x+1)}= \frac{x+2x+1-2}{(x-1)(x+1)}= \frac{3x-1}{(x-1)(x+1)}$$