$$S= \sum\limits_{k=0}^{20}(x_{k}+ y_{k} )= \sum\limits_{k=0}^{20}x_{k}+ \sum\limits_{k=0}^{20}y_{k}= ( 8 + \sum\limits_{k=1}^{20}x_{k})+ (\sum\limits_{k=0}^{18} y_{k}+ y_{19}+y_{20})$$
$$S = (8 +42) + (-4 -8 +4)=42$$


----

$$\sum\limits_{k=11}^{20}3x_{k}- 2y_{k}= 3\left(\sum\limits_{k=11}^{20}y_{k}\right)- 2(5) = \left(\sum\limits_{k=1}^{20}x_{k}- \sum\limits_{k=1}^{10}x_{k}\right) - 10 = (30 - 42) - 10= -22$$

----






$$\int_{-2}^{3} \frac{1}{x^{4}}dx= - \frac{1}{3x^{3}} + C$$
$$\text{Minor problem, divergent at 0.}$$
---

$$\frac{1002}{7-2000}=-0.5028$$


---

$$\text{Converges at } \frac{a}{1-r}= \frac{6}{0.1}=60$$


---

$$\text{Using growth rates, } \pi^{n} \text{ is growing faster, so } \lim\limits_{n \to \infty} \frac{\pi^{n}}{3^{n+1}}= \infty, \text{meaning divergent}$$

---

$$\cancel{s_{0}= \frac{2}{7}}, S_{1}= \frac{3}{5}, S_{2} = \frac{4}{3}, S_{3}= \frac{5}{1}, S_{4}= \frac{6}{-1} $$

$$\lim\limits_{n \to \infty} \frac{n+2}{7-2n}= \frac{1}{-2}= \frac{-1}{2} \text{ converges there!}$$


---


$$\sum\limits_{n=1}^{\infty}\frac{(-3)^{n-1}}{4^{n}}= \sum\limits_{n=1}^{\infty}  \frac{-3^{n}*(-3)^{-1}}{4^{n}}= \sum\limits_{n=1}^{\infty } -\frac{1}{3}(\frac{-3^{n}}{4^{n}})=\sum\limits_{n=1}^{\infty} \frac{-1}{3}(\frac{-3}{4})^{x} =  $$
$$\sum\limits_{l=0}^{\infty} - \frac{1}{3}( - \frac{3}{4})^{l+1} =  \sum\limits \frac{-1}{3}(\frac{-3}{4})^{l}(\frac{-3}{4})^{1}$$
$$\sum\limits_{l=0}^{\infty} \frac{1}{4}( \frac{-3}{4})^{l}= \frac{\frac{1}{4}}{1+ \frac{3}{4}}=  \frac{1}{7}$$
