
$\Delta x = 89.25$
$y_{o}=6.5$
$\theta = 45$
$y_{f}=10$

Trying to find $v_{o}$

$a_{x}(t)=0$
$v_{x}(t)=v_{x,o}$
$x(t)=x_{o}+v_{x}(t)$


Y component
$a_{y}(t)=-g$
$v_{y}(t)=v_{y,o} -gt$
$y(t)=y_{i}+v_{y,o}t- \frac{1}{2}gt^{2}$

$v_{y,o} = v_{o}*\sin(\theta)$
$v_{x,o}=v_{o}*\cos(\theta)$


So we end up with

$x(t)=x_{o}+v_{o}\cos(\theta)t$
$y(t)=y_{i}+v_{o}\sin(\theta)t - \frac{1}{2}gt^{2}$
We could say we're trying to find the final, so

$x_{f}=x_{o}+v_{o}\cos(\theta)t$
$y_{f} =y_{i}+v_{o}\sin(\theta)t - \frac{1}{2}gt^{2}$
Two equations, two unknowns

$v_{o}=\frac{x_{f}-x_{o}}{\cos(\theta)t}$

$y_{f}=y_{i}+ (\frac{x_{f}-x_{o}}{\cos(\theta)t})\sin(\theta)t - \frac{1}{2}gt^{2}$
Solve that for t

$y_{f}-y_{i}= \tan(\theta)(x_{f}-x_{o})- \frac{1}{2}gt^{2}$
$\sqrt{-\frac{y_{f}-y_{i}- (\tan(\theta)(x_{f}-x_{o}))}{\frac{1}{2}g}} = t$

Plug and chug all THOSE shenanigans, you end up with 2.315 seconds for $t$

Plugging that back in to the equation for $v_{o}$, initial velocity of 54.521 ft/s





