#notes #math111 #math #calc



# Implicit Differentiation
- Say what the hell that means
- Calculate $\frac{dy}{dx}$ for an implicitly defined function
- use it to do shenanigans



Solve $x^{2}+y^{2}=25$ for some shenanigans

$y=\pm\sqrt{25-x^{2}}$
The plus is the top half of the circle, the - is the bottom half of the circle 

use $y=\sqrt{25-x^2}$
to find $\frac{dy}{dx}$

$y=(25-x^{2})^{\frac{1}{2}}$

$y'=\frac{1}{2}(25-x^{2})^{\frac{-1}{2}}-2x$

$y'=\frac{-x}{\sqrt{25-x^2}}$

$\Big|_a^b$

Maybe we can't actually solve for y, and we can't get the explicit differentiation

Using the equation $x^2+y^{2}=25$

1. Differentiate both sides with respect to x

$$\frac{d}{dx}(x^{2}+y^{2})=\frac{d}{dx}(25)$$
$$\frac{d}{dx}(x^{2}) + \frac{d}{dx}(y^{2)} =\frac{d}{dx}(25)$$

Those ones with just x are *awesome*, we can do whatever we want with those ones
on the other hand, when we see a y around, we have a problem
- We gotta ponder that $y=f(x)$
- Which, in that case, we need to conjure up the chain rule

gots to find
$\frac{d}{dx}(y^{2})$
which is the same thing as $$\frac{d}{dx}((f(x))^{2}) = 2(f(x))*f'(x)= 2y* \frac{dy}{dx}$$
so hip hopping back up

$$2x + 2y * \frac{dy}{dx}=0$$
2. Someone (if they're cringe) might ask us to solve for dy/dx 
$$2x + 2y \frac{dy}{dx}=0 \ \ = \ \ 2y \frac{dy}{dx}=-2x$$

$$\frac{dy}{dx}=\frac{-x}{y}$$

3. Plug in at a point $(x,y)$ to find the slope at that point
$$\frac{dy}{dx}\Big|_{(3,4)} = \frac{-3}{4}$$



If we want to find where it's horizontal, dy/dx = 0, and you can just solve for that

Find the equation of the tangent line to $2x^{3}+2y^{3}=9xy$ at the point (2,1)

We gonna need to implicit this lil fella

$$\frac{d}{dx}(2x^{3})+ \frac{d}{dx} (2y^{3}) = \frac{d}{dx}(9xy)$$
- That first one is easy
	- Second one is a wonderful chain rule problem
		- Third one is an icky gross product rule trying to sneak its way into being a reasonable function with friends
party time

$$6x^{2} + 2*3y^{2}* \frac{dy}{dx}=9x \frac{dy}{dx} + 9y$$
 

that algebra is awful and I'm going to represent $\frac{dy}{dx}$ with a $d$ just to make my life easier
$$6y^{2}d -9xd = 9y-6x^{2}$$
$$\frac{dy}{dx}(6y^{2}-9x) = 9y - 6x^2$$$$\frac{dy}{dx}=\frac{9y-6x^2}{6y^2-9x}$$
So now we have a somewhat reasonable equation, so let's go plug in $(2,1)$

$$\frac{dy}{dx}\Big|_{(2,1)} \frac{9(1)-6(2)^{2} }{6(1)^{2}-9(2)} = \frac{9-24}{6-18}=\frac{-15}{-12}=\frac{5}{4}$$



$$y-1=1.25(x-2)$$
