#notes #math111 #math #calc

- Horizontal asymptotes are limits to infinity
- Vertical asymptotes are to a number, where the answer is infinity
#### Example
- Find all horizontal and vertical asymptotes for $f$ and justify by showing the appropriate limit
#### ok other example rq
Find horizontal asymptotes, look at what happens at infinity
$$f(x) = \frac{x}{\sqrt{x^2+1}}$$
$\sqrt{x^{2}}$ is the same thing as $|x|$ 

do to this
$$\lim\limits_{x \to \infty}  \frac{x}{\sqrt{x^2+1}}=\lim\limits_{x \to \infty}\frac{x}{\sqrt{x^{2}(1+\frac{1}{x^{2}})}}=\lim\limits_{x \to \infty}\frac{x}{\sqrt{x^{2}}+\sqrt{1+\frac{1}{x^2}}}=\lim\limits_{x \to \infty}\frac{x}{|x|\sqrt{1+\frac{1}{x^2}}}=\lim\limits_{x \to \infty}\frac{x}{x\sqrt{\frac{1}{x^{2}}}}=\lim\limits_{x \to \infty}\frac{1}{\sqrt{1+1/x^{2}}}$$
$$\lim\limits_{x \to \infty}\frac{1}{\sqrt{1+0}}=1$$
#### The real example
$$f(x) = \frac{x^{3}-5x^{2}+6x}{x^{4}-4x^{2}}$$
Since f is rational, we only have 1 horizontal asymptote
Only look at $\lim\limits_{x \to \infty}f(x)$ $$=\lim\limits_{x \to \infty}\frac{x^{3}}{x^{4}}=\lim\limits_{x \to \infty}\frac{1}{x}=0$$
Horizontal asymptote at $y=0$
Vertical asymptote need some work, so we gotta figure out what the hell $a$ is first
Potential vertical asymptotes when the denominator is 0
$$x^4-4x^2=(x^2)(x^2-4)=0$$
So we have roots at $\pm$ 2 and 0
Now, the sticky wicket is that this does NOT mean we have vertical asymptotes, we gotta go check 
Lets get to checking them
$$\lim\limits_{x \to 2^+}\frac{x^3-5x^2+6x}{(x^2)(x-2)(x+2)}=\lim\limits_{x \to 2^+}\frac{(x)(x^2-5x+6)}{x^2(x-2)(x+2)}=\lim\limits_{x \to 2^+}\frac{(x)(x-2)(x-3)}{x^2(x-2)(x+2)}\lim\limits_{x \to 2^+}\frac{(x)(x-3)}{x^2(x+2)}=\lim\limits_{x \to 2^+}\frac{x-3}{x(x+2)}=$$
$$\lim\limits_{x \to 2^+}-\frac{1}{8}$$
Oh hey, that's not $\infty$, (or -$\infty$ ), so that's just a hole. Womp womp. 

$$\lim\limits_{x \to -2^{+}}f(x)=\frac{(x-3)}{x(x+2)}=\frac{-5}{0}$$
Which tells us the limit Does Not Exist, which isn't much good when you're trying to figure out an asymptote
Now, the real wicket is it $+\infty$ or $-\infty$ $$\lim\limits_{x \to -2^+}\frac{x-3}{(x)(x+2)}=\frac{-5}{+smol(-)}=\frac{-}{-}=+$$
Soooooo, $\lim\limits_{x \to -2^+}f(x)=+\infty$

