#notes #math225 #math 

## Still in Laplace land
$$
\mathcal{L}\{c_{1}f(t)+c_{2}g(t)\}=c_{1}F(s)+c_{2}G(s)
$$
- Is what we were doing last time, generally covering linearity and such where constants pop out and you can add functions together in integral shenanigans.
### Shift
$$
\mathcal{L}\{e^{at}f(t)\}=\int_{0}^{\infty}e^{at}f(t)e^{-st}dt
$$
$$
= \int_{0}^{\infty}e^{(a-s)t}f(t)dt
$$
$$
w = s-a, dw = ds
$$
$$
= \int_{0}^{\infty}e^{-wt}f(t)dt
$$
- That sure seems to just deadass look like the definition of a Laplace transform, where we use w instead of s 
$$
\int_{0}^{\infty}e^{-wt}f(t)dt = F(w)=F(s-a)
$$
$$
\mathcal{L}\{e^{at}f(t)\}=F(s-a)
$$
- This is one of two shift properties of (Laplace, but also Fourier) integral transforms
## Inverse Transform
- if $\mathcal{L}\{f(t)\}=F(s)$, then $\mathcal{L}^{-1}\{F(s)\}=f(t)$
$$
\mathcal{L}^{-1}\left\{ \frac{1}{s^{2}} \right\}
$$
- We go look at the formula sheet, so the inverse of $\frac{1}{s^{2}}$ is $t$
$$
\mathcal{L}^{-1}\left\{ \frac{1}{s+3} \right\}= e^{-3t}
$$
$$
e^{at}\stackrel{ \mathcal{L}\{\} }{ \implies }= \frac{1}{s-a}
$$
- Sometimes, you unfortunately have to do some algebra to get our function into a form on the sheet
	- Sometimes it's really simple and you just multiply and it's great, but otherwise...
	1. Sometimes you have to do partial fractions
	2. Sometimes you must complete the square
---
$$
\mathcal{L}^{-1}\left\{ \frac{s}{s^{2}+2s-3} \right\} = \mathcal{L}^{-1}\left\{ \frac{s}{(s+3)(s+1)} \right\}
$$
$$
\frac{s}{(s+3)(s-1)}= \frac{A}{(s+3)}+\frac{B}{(s-1)}
$$
$$
As-A+Bs+3B=s
$$
$$
A+B=1, -A+3B = 0
$$
$$
B= \frac{1}{4}, A = \frac{3}{4}
$$
$$
\frac{3}{4 }* \frac{1}{s+3} + \frac{1}{4 } * \frac{1}{s-1}
$$
$$
\mathcal{L}^{-1}\{\} = \frac{3}{4}e^{-3t} +\frac{1}{4}e^{t}
$$
---

$$
\mathcal{L}^{-1}\left\{ \frac{2s-6}{s^{2}+9} \right\} = \mathcal{L}^{-1}\left\{ \frac{2s}{s^{2}+9}-\frac{6}{s^{2}+9} \right\}
$$
- We've got a couple interesting formulas, notably 13, which has $\cos kt\implies \frac{s}{s^{2}+k^{2}}$, and 14 has $\sin kt\implies \frac{k}{s^{2}+k^{2}}$
$$
\mathcal{L}^{-1}\left\{ \frac{2s}{s^{2}+9} \right\}= 2 \mathcal{L}^{-1}\left\{ \frac{s}{s^{2}+9} \right\}= 2\cos(3t)
$$
$$
\mathcal{L}^{-1}\left\{ -\frac{6}{s^{2}+9} \right\}=-6\mathcal{L}^{-1}\left\{ \frac{1}{s^{2}+9} * \frac{3}{3}\right\}= -\frac{6}{3}\{\}= -2 \left\{ \frac{3}{s^{2}+9} \right\}
$$
$$
\mathcal{L}^{-1}\left\{ \frac{2s-6}{s^{2}+9} \right\}=2\cos(3t)-2\sin(3t)
$$
-----
$$
\mathcal{L}^{-1}\left\{ \frac{3s+2}{s^{2}-6s+18} \right\}
$$
- None of the really obvious options are options here, so we're completing the square in the denominator (divide middle by 2 and square it)
$$
\frac{3s+2}{s^{2}-6s+9-9+18}
$$
$$
\frac{3s+2}{(s-3)^{2}+9}
$$
- Some fun formulae from the sheet:
	17. $e^{at}\cos kt\implies \frac{s-a}{(s-a)^{2}+k^{2}}$
	18. $e^{at}\sin kt\implies \frac{k}{(s-a)^{2}+k^{2}}$
$$
3\left[  \frac{s}{(s-3)^{2}+9} \right]+\frac{2}{(s-3)^{2}+9}= 3\left[ \frac{s}{(s-3)^{2}+9}-\frac{3}{(s-3)^{2}+9} + \frac{3}{(s-3)^{2}+9}\right] + \frac{2}{(s-3)^{2}+9}
$$
$$
3\left[ \frac{s-3}{(s-3)^{2}+9} \right]+ \frac{1}{(s-3)^{2}+9}*\left( \frac{3}{3)} \right)=3e^{3t}\cos(3t)+\frac{11}{3}e^{3t}\sin(3t)
$$
