#notes #math225 #math 

## Still doing second order homogeneous
- Which were, to recap, of the form $$
ay''  + by' +cy = 0
$$
- From the characteristic equation, we can end up with two real roots $m_{1}$ and $m_{2}$, which gives you the general solution $y=c_{1}e^{m_{1}x}+c_{2}e^{m_{2}x}$
	- You can also end up with one real (repeated) root, $m_{1}$, which pops out the general solution $y=c_{1}e^{m_{1}x}+c_{2}xe^{m_{1}x}$
- We can also have complex conjugate roots!
#### Leading in with an example
$$
y''+4y'+7y=0
$$
- Soooo... we're going to use the characteristic equation. $$
m^{2}+4m+7
$$
- That looks rather the far side of factorable, so we're going to pop in ol tried and true, the quadratic formula
$$
m = -\frac{4\pm \sqrt{ 16-28 }}{2}= \frac{-4\pm \sqrt{ -12 }}{3}= -\frac{4\pm \sqrt{ -(4)(3) }}{2}= -\frac{-4\pm 2\sqrt{ -3 }}{2} =-2\pm i\sqrt{ 3 }
$$
- So our solution then becomes the properly ugly $$
y = c_{1}e^{(-2+i\sqrt{ 3 })x}+c_{2}e^{(-2-i\sqrt{ 3 })x}
$$
- This is certainly an answer of all time. However, we won't write our answers with these complex shenanigans.
$$
y=c_{1}e^{-2x}e^{-\sqrt{ 3 }x} + c_{2}e^{-2x}e^{-i\sqrt{ 3 }x}
$$
- If you suppose the characteristic equation is $a\pm bi$, then $$
y = c_{1}e^{(a+bi)x}+c_{2}e^{(a-bi)x}
$$
- Since these two functions are linearly independent, sums and/or differences of these terms are also solutions to the differential equation.
	- For example, $y_{1}+y_{2}$ is a solution that gives you $e^{(a+ib)x}+e^{(a-ib)x}$
		- That's, believe it or not, a form of cosine. Go tap ol' Euler in [[Compilations/Calc + Diffeq/MATH225 Comp/MATH225 - 2025-02-24]]
			- You get things like $\cos(x)=\frac{e^{-ix}+e^{ix}}{2}$
		- So this becomes $2e^{ax}(\cos(bx))$
	- So if we then have $e^{ax}[e^{ibx}-e^{-ibx}]$
		- and then $\sin(x)= \frac{1}{2i}[e^{ix}-e^{-ix}]$
		- Which then gives you $2ie^{ax}\sin(bx)$
- So then combing together the general solution is going to be $$
y=c_{1}e^{ax}\cos(bx)+c_{2}e^{ax}\sin(bx)
$$
----
-  Complex conjugate roots $m=a\pm ib$ will be written as $$
y = c_{1}e^{ax}\cos(bx)+c_{2}e^{ax}\sin(bx)
$$
---
#### Brief Aside
- We can also write the solution as $y = c_{1}e^{ax}\cos(bx-\phi)$
	- This is just trig shenanigans because sine is just cosine with a phase shift, so this is collapsing it down to $c_{1}$ and $\phi$ as our constants.

### More Example
$$
\frac{d^{2}y}{d\theta^2}+y=0
$$
$$
y\left( \frac{\pi}{3} \right)=0,y'\left( \frac{\pi}{3} \right)=2
$$
- Character equation is going to be $m^{2}+1=0\implies m=\pm i$
	- Boy howdy, that sure looks like a complex conjugate root.
	- These roots have no real part, or $a=0$
$$
y=c_{1}\cos(\theta)+c_{2}\sin(\theta)
$$
$$
y\left( \frac{\pi}{3} \right)=0=c_{1}\cos\left( \frac{\pi}{3} \right)+c_{2}\sin\left( \frac{\pi}{3} \right)
$$
$$
0=\frac{1}{2}c_{1}+c_{2}\frac{\sqrt{ 3 }}{2}
$$
$$
y' = -c_{1}\sin \theta+c_{2}\cos(\theta)
$$
$$
y'\left( \frac{\pi}{3} \right)=c_{1}\sin\left( \frac{\pi}{3} \right)+c_{2}\cos\left( \frac{\pi}{3} \right)
$$
$$
2= \frac{c_{1}\sqrt{ B }}{2}+\frac{1}{2}c_{2}
$$
$$
0=\frac{1}{2}c_{1}+c_{2} \frac{\sqrt{ 3 }}{2}
$$
$$
2= -\frac{\sqrt{ 3 }}{2}c_{1} + \frac{1}{2}c_{2}
$$
- Do a little simplifying
$$
0 = c_{1}+\sqrt{ 3 }c_{2}
$$
$$
4=-\sqrt{ 3 }c_{1}+c_{2}
$$
$$
c_{1}=-\sqrt{ 3 }\ c_{2}
$$
$$
4 = 3c_{2}+c_{2}, 4 = 4c_{2}, \boxed{c_{2} = 1}
$$
$$
\boxed{
c_{1}= -\sqrt{ 3 }
}
$$
- So the solution to the IVP is going to be $y=-\sqrt{ 3 }\cos(\theta)+\sin(\theta)$
---
- Fun aside, we can use the characteristic equation with higher order ODES, but you need to solve cubics or quartics, which, been a minute.
