#notes #math213 #math #calc

## more 15.2 (TPT)
- couple general examples

$$\lim\limits_{(x,y) \to (0,0)} [ \frac{xy}{x^{2}+ y^2}]$$
- Plug in will fail you. Algebra will fail you. L'Hopital is dead.
- In this case, let's try the x axis, $y=0$

$$\lim\limits_{(x,y) \to (x,0)}|\frac{xy}{x^{2}+y^{2}}| $$
$$= \frac{0}{x^{2}+0}=0$$
$$\lim\limits_{(x,y) \to (0,y)} | \frac{xy}{x^{2}+y^{2}}|$$
$$\frac{0}{y^{2}}=0, \text{ Sadly, }0=0$$
Trying $y=x$
$$\lim\limits_{(x,y) \to (0,0)}\left[ \frac{xy}{x^{2}+y^{2}}\right]$$
$$\lim\limits_{n \to \infty} \frac{(x)(x)}{x^{2}+x^{2}}$$
$$\lim\limits_{n \to \infty} \frac{x^{2}}{2x^{2}}= \frac{1}{2}$$
By TPT limit Does Not Exist


----

- So this is fun, but shooting individual paths is kind of tiring
- So just choose $y=mx$ for literally all the lines going through the origin

$$\lim\limits_{(x,y) \to (0,0)} \frac{xy}{x^{2}+ y^{2}}= \lim\limits_{x \to 0}\frac{(x)(mx)}{(x^{2})+ (mx)^{2}}$$
$$\lim\limits_{x \to 0}\frac{mx^{2}}{x^{2}(1+m^{2})}$$
$$\lim\limits_{x \to 0} \frac{m}{1+m^{2}}= \frac{m}{1+m^{2}}$$

---

#### where lines fail.
$$\lim\limits_{(x,y) \to (0,0)} \frac{3xy^{2}}{x^{2}+ y^{4}}$$
Trying $y=mx$

$$\lim\limits_{(x,y) \to (0,0)\text{ along y=mx}}\frac{3xy^{2}}{x^{2}+y^{4}}$$
$$\lim\limits_{x \to 0} \frac{3x(mx)^{2}}{x^{2}+ (mx)^{4}}$$
$$\lim\limits_{x \to 0}\frac{3x^{3}m^{2}}{x^{2}(1+m^{4}x^{2})}$$
$$\lim\limits_{x \to 0}\frac{3xm^{2}}{1+m^{4}x^{2}}=0$$
- Pro gamer parabola advice:
	- Consider the function that you're working with 
	- In this case, let's try $x=y^{2}$

$$\lim\limits_{(x,y) \to (0,0)\text  x= y^{2}} \frac{3xy^{2}}{x^{2} + y^{4}}$$
$$\lim\limits_{x \to 0} \frac{3x(x)}{x^{2}+ x^{2}}= \lim\limits_{x \to 0} \frac{3x^{2}}{2x^{2}}= \frac{3}{2}$$
- Which means our limit does not exist by two path test.

---

### Polar Shenanigans
- only do this if you have to.

$$x=r\cos\theta, y = r\sin\theta, x^{2}+y^{2}=r^{2}$$
- If we were to do be doing a limit as $(x,y)\to(0,0)$
	- Radius would be-a shrinking, $r\to 0^{+}$

$$\lim\limits_{(x,y) \to (0,0)}\frac{x^{3}-y^{3}}{x^{2}+ y^{2}}$$
$$\lim\limits_{(x,y) \to (0,0)}\frac{(r\cos\theta)^{3}- (r\sin\theta)^{3}}{r^{2}}$$
$$\lim\limits_{r \to 0^{+}}\frac{r^{3}(\cos^{3}\theta -\sin^{3}\theta)}{r^{2}}$$
$$\lim\limits_{r \to 0^{+}} r(\cos^{3}\theta - \sin^{3}\theta)= 0$$

----

# Partial Derivatives
- Essentially the way the cookie crumbles is that you look at each rate of change individually ofr multivariable functions
- We need to consider direction when discussing RoC in $\mathbb{R}^{3}$
	- $f_{x}$ is the partial of $f$ with respect to $x$
	- $f_{y}$ is the partial of $f$ with respect to $y$
- The partial derivative of $f$ with respect to $x$ at a point $(a,b)$ is given by$$f_{x}(a,b) = \lim\limits_{h \to 0}\frac{f(a+h,b)-f(a,b)}{h}$$
- This fine piece of bullshit is the instantaneous rate of change in the $x$ direction
$$f_{y}(a,b) = \lim\limits_{h \to 0} \frac{f(a,b+h) - f(a,b)}{h}$$
- That's the instantaneous rate of change in the $y$ direction. Happy day.

$$f = \lim\limits_{h \to 0} \frac{(x+h)^{2}y - x^{2}y}{h}= \lim\limits_{h \to 0}\frac{x^{2}y + 2xhy + yh^{2}- x^{2}y}{h}$$
$$\lim\limits_{h \to 0}2xy + yh$$
$$f_{x}= 2xy$$
---
It's just going to be $x^{2}!$ god damn it! why must we *suffer*

$$f_{y}= \lim\limits_{h \to 0 }\frac{x^{2}(y+h)-x^{2}y}{h}$$
$$\lim\limits_{h \to 0 }\frac{\cancel{x^{2}y} + x^{2}\cancel{h}-\cancel{x^{2}y}}{\cancel{h}}$$
$$\lim\limits_{h \to 0} x^{2}= x^{2} $$
