#notes #math213 #math #calc

- Last time we were doing the limit definition
	- can we please make this easier

## Notation
- Two kinds of notation:
	- Newtonian
		- $f_{x}$ and $f_{y}$ is just your function with subscripts 
	- Leibniz
		- $\frac{\partial f}{\partial x}$ and $\frac{\partial f}{\partial y}$
	- If defined at $(a,b)$
		- $f_{x}(a,b)$, $\frac{\partial f}{\partial x}\Big|_{(a,b)}$
## Computing Partials
1. Use the limit definition
	1. (I really don't want to)
2. Or derivative rules! (with a twist)

#### Example
- Use derivative rules to compute $f_{x}$ and $f_{y}$
$$f(x,y)= \sin(xy)+ 3x^{2}+ 2xy^{3}-\ln(y)$$
$$f_{x}= \cos(xy)*y + 6x + 2y^{3}- 0$$
$$f_{y}= \cos(xy)x + 0 + 6xy^{2}- \frac{1}{y}$$

#### again!
$$f(x,y) = (2x-y^{3})^{4}$$
$$f_{x}=4(2x-y^{3})^{3}*2$$
$$f_{y}= 4(2x-y^{3})^{3}*-3y^{2}$$

----

## Derivative rules will hold for 3 or more variables!
ie, $h(x,y,z,w)$ gives you $h_{x}, h_{y}, h_{z}, \text{ and } h_{w}$

---

## beyond the first order (ie, second order


$$\frac{\partial}{\partial x} \left[ \frac{\partial f}{\partial x}\right]= \frac{\partial^{2}f}{\partial x^{2}} = f_{xx} $$
$$\frac{\partial}{\partial x} \left[\frac{\partial f}{\partial y}\right]$$
Read from the inside out for ~~leibniz~~ both!

#### Find all 2nd order partials
$$ x^{3}+ x^{2}y^{2}- 2y^{2}+ \frac{x}{y}$$
$$f_{x}= 3x^{2}+ 2xy^{2}+ \frac{1}{y}$$
$$f_{xx}= 6x + 2y^{2}$$
$$f_{xy} = 4xy - \frac{1}{y^{2}}$$
$$f_{y}= 2yx^{2} - 4y   - \frac{x}{y^{2}}$$
$$f_{yy}= 2x^{2}-4 +\frac{2x}{y^{3}}$$
$$f_{yx} = 4xy  - \frac{1}{y^{2}}$$
In calc 3, $f_{yx}=f_{xy}$
- This is not true for everything! Just most things you're going to do in calc 3 since we have easy domains


### Clairaut's Theorem
- If $f$ is defined on a domain, $D$ in $\mathbb{R}^{2}$, and both $f_{yx}$ and $f_{xy}$ are continuous on a domain, then they're the sameses


$$f(x,y,z)= e^{xyz}+ \sin(\frac{x^{2}- \ln(y)}{^{2y}})$$
$$f_{y}= xz*e^{yxz} + \cos(\frac{x^{2}- \ln(y)}{e^{2y}})* (\frac{-\frac{2y}{y} - 2(x^{2}- \ln(y))}{y^{2}})$$
- Either I missed something or that is just god awful

$$f_{yz}= x*e^{yzx}+ x^{2}zye^{yzx}+ 0$$
$$f_{yzy}= x^{2}z*e^{yxz}+ x^{3}$$
I did in fact fucking miss something, you can prove that there's a domain and then you can do z first

$$D := \{x,y,z \in \mathbb{R} \mid y > 0\}$$
We can apply that theorem and do 

$$f_{zyy}= yxe^{xyz}+ 0$$
$$f_{yy}= x(e^{xyz})+xy(xze^{xyz})$$
$$f_{yy}= x e^{xyz} + (x^{2}yz)*e^{xyz}$$
$$f_{yyy}= x(xze^{xyz})+ (x^{2}z)(e^{xyz}) + (x^{2}zy )(xze^{xyz})$$
- I was, for the record, doing that right

----

## Activity Stuff

1. Find $f_{x}$ and $f_{y}$ for 
$$f(x,y) = y^{3}\sin(4x)$$
$$f(x,y) = \sqrt{4+x^{2}+y^{2}}$$
2. Verify $f_{xy}= f_{yx}$ for a domain D for $f(x,y)= 3x^{2}y^{-1}-2x^{-1}y^{2}$
