#notes #math213 #math #calc


So back in calc 1, we did like 
$$f(g(x))= f'(g(x))*g'(x)$$
- Which, notably, only really deals with one variable ($x$, in this case) 

Now in this fresh hell
$$z= f(x,y)$$

### Chain rule for 1 Independent Variable
- Let $z$ be a differentiable function on its domain where x and y are differentiable with respect to $t$ along an interval I
$$\frac{dz}{dt}= \frac{\partial z}{\partial x}\left[\frac{dx}{dt}\right]+ \frac{\partial z}{\partial y}\left[\frac{dy}{dt}\right]$$
- Note, in this case, $t$ is the only independent variable, even if z is defined as of x and y.
- x and y are known as intermediate variables

#### Example
Find $\frac{dz}{dt}$ where $z=x\sin{y}$ and $x=t^{2}$, $y=4t^{3}$

$$\frac{dz}{dt}= \frac{\partial z}{\partial x}\left[\frac{dx}{dt}\right]+ \frac{\partial z}{\partial y}\left[\frac{dy}{dt}\right]$$
$$\frac{\partial z}{\partial x}= \sin y$$
$$\frac{\partial z}{\partial y}= x\cos y$$
$$\frac{dx}{dt}= 2t$$
$$\frac{dy}{dt}= 12t^{2}$$
$$\frac{dz}{dt}= (\sin y)(2t) + (x\cos y) (12t^{2})$$
$$\frac{dz}{dt}= (2t)\sin(4t^{3}) + 12t^{4}\cos(4t^{3})$$

### Tree Diagrams
- Tree diagrams exist to extend chain rule to more intermediate variables.

$$\frac{dw}{dt}= \sqrt{x^{2}+ y^{2}+ z^{2}}$$
for $x=\sin t, y = \cos t, z = \cos t$
$$\frac{\partial w}{\partial x}= x(x^{2}+y^{2}+z^{2})^{-\frac{1}{2}}$$
$$\frac{\partial w}{\partial y}= y(x^{2}+y^{2}+z^{2})^{-\frac{1}{2}}$$
$$\frac{\partial w}{\partial z}= \frac{\partial w}{\partial x}= z(x^{2}+y^{2}+z^{2})^{-\frac{1}{2}}$$

$$\frac{dx}{dt}= \cos t$$
$$\frac{dy}{dt}= -\sin t$$
$$\frac{dz}{dt}= -\sin t$$
$$\frac{dw}{dt}= \frac{1}{\sqrt{x^{2}+ y^{2}+ z^{2}}}( x\cos t - y\sin t - z \sin t)$$
$$= \frac{1}{\sqrt{\sin^{2}t + 2\cos^{2}t}}( \cancel{ \sin\cos t - \cos t \sin t}- \cos t\sin t)$$
$$= \frac{\cos t \sin t}{\sqrt{\sin^{2}t + 2\cos^{2}t}}$$

## Implicit Differentiation
- Let $f$ be differentiable on its domain and suppose $F(x,y)=0$ defines $y$ as a function of $x$ $\therefore F(x,y) = F(x,y(x))$
- $$\frac{dy}{dx}= \frac{-F_{x}}{F_{y}}$$
### example
Find $\frac{dy}{dx}$ for $$\sin(xy) + \pi y^{2}-x = 0$$
$$F_{x}= y\cos(xy)-1$$
$$f_{y}= x\cos(xy)+2\pi y$$
$$\frac{dy}{dx}= - \frac{y\cos(xy)-1}{x\cos(xy)+2\pi y}$$
- as long as they're both 0 this is fine

- Note: implicit differentiation holds when finding partials 

#### example 2: the exampling
If $w=f(x,y,z)$

Let's find $\frac{\partial t}{\partial x}$ and $\frac{\partial x}{\partial y}$
of $$xy + z = \cos(xz)$$
$$xy + z -\cos(xz) = 0$$
$$\frac{\partial z }{\partial x}= \frac{- F_{x}}{F_{z}}= -\frac{(y + z\sin(xz))}{1 + x\sin(xz)}$$
$$\frac{\partial x}{\partial y}= - \frac{F_{y}}{F_{x}}= \frac{-x}{y + z\sin(xz)}$$

### exampl'nt
$$z = 2x^{2}+ y^{2}+ 1$$
and curve in the xy plane given by $$x=1+\cos(t), y=\sin t, 0 \leq t \leq 2\pi$$Find where $z$ is increasing, aka, find $\frac{dz}{dt} > 0$
$$\frac{dz}{dt}= 4x ( -\sin(t)) + (2y)(\cos(t))$$
$$\frac{dz}{dt}= 4(1+\cos(t))(-\sin(t)) + 2(\sin t) (\cos(t))$$
$$-2\sin(t)\left[2(1+\cos t) - \cos t\right]  $$
$$= -2 \sin t[ 2 + \cos(t)] $$
$$\text{ When is sin negative? }\pi < t < 2\pi$$
$$\text{ When is cos positive? } 0 < t < 2\pi$$
So our final answer is just $\pi < t < 2\pi$

