#notes #phgn200 #physics

$$u= u_{e}+ u_{b}$$
$$u_{e}= \frac{1}{2}\epsilon_{0}E^{2}$$
$$u_{b}= \frac{B^{2}}{2\mu_{0}}$$
$$u=\frac{1}{2}\epsilon_{0}E^{2}+ \frac{B^{2}}{2\mu_{0}}$$
$$E=\frac{B}{\epsilon_{0}\mu_{0}c}$$
$$E =\frac{B}{\epsilon_{0}\mu_{0}(\sqrt{\epsilon_{0}\mu_{0}})}$$
$$\frac{1}{2}\epsilon_{0}E^{2}= \frac{1}{2}\epsilon_{0}( \frac{B^{2}}{\epsilon_{0}^{2}\mu_{0}^{2}\epsilon_{0}\mu_{0}})$$
$$\frac{1B^{2}}{2\epsilon_{0}^{2}\mu_{0}^{3}}+ \frac{B^{2}}{2\mu_{0}}$$
---

$$I_{avg}= u_{rms}c$$
$$u = E^{2}\epsilon_{0}$$
$$u = \left(\frac{E_{0}}{\sqrt{2}}\right)^{2}\epsilon_{0}*c$$