#math #math111 
$$\lim\limits_{x \to 4}\frac{(x+2)^{2}-9x}{4-x}=\lim\limits_{x \to 4}\frac{x^2-5x+4}{4-x}=\lim\limits_{x \to 4}\frac{(x-4)(x-1)}{4-x}*-1=\lim\limits_{x \to 4}\frac{(x+4)(-x+1)}{4+x}=\lim\limits_{x \to 4}x-1=-3$$

$$\lim\limits_{x \to 0}\frac{x}{\sqrt{6x+1}-1}*\frac{\sqrt{6x+1}+1}{\sqrt{6x+1}+1}=\lim\limits_{x \to 0}\frac{(x)(\sqrt{6x+1}+1)}{6(x)}=\lim\limits_{x \to 0}\frac{\sqrt{6x+1}+1}{6}=\lim\limits_{x \to 0}\frac{2}{6}=\lim\limits_{x \to 0}\frac{1}{3}=\frac{1}{3}$$
$$\lim\limits_{x \to -4}\frac{x^2+4x}{x^3+2x^2-8x}=\lim\limits_{x \to -4}\frac{x(x+4)}{x(x^2+2x-8)}=\lim\limits_{x \to -4}\frac{(x)(x+4)}{(x)(x+4)(x-2)}=\lim\limits_{x \to -4}\frac{1}{x-2}=-\frac{1}{6}$$
3x-4ln(2) = ln(14)

(5x+2)\*ln(2) = ln(18)

$$\frac{\ln{18}}{5*\ln{2}}+\frac{2}{5}$$

$$e^{11k}=5$$


------------

$$4*2^{x-5}=12 \ , /4$$
$$2^{x-5}=3$$
$$(x-5)\ln(2)=\ln(3)$$
$$x-5=\frac{\ln(3)}{\ln(2)}$$
$$x=5+\frac{\ln(3)}{\ln(2)}$$


---
$$\ln(x-1)+\ln(x+1)=\ln(12)$$
$$(x-1)(x+1)=12$$
$$x^2-1=12$$
$$x=\sqrt{13}$$
----
$$\lim\limits_{x \to \infty}\frac{e^x}{1+e^{-x}}=\lim\limits_{x \to \infty}\frac{\infty}{1+0}=\lim\limits_{x \to \infty}\infty=\infty$$
------
$$\lim\limits_{x \to \infty}\frac{e^x}{1+e^{-x}}=\lim\limits_{x \to \infty}\frac{0}{1+\infty}=\lim\limits_{x \to \infty}0=0$$

-------
$$\lim\limits_{x \to -\infty}\frac{3x^2+4x}{x+1}=\lim\limits_{x \to -\infty}\frac{(x)(3x+4)}{x+1}=\lim\limits_{x \to \infty}\frac{-\infty*-\infty}{-\infty}=-\infty$$
$$\lim\limits_{x \to -\infty}\frac{-\infty^2-\infty}{-\infty}=\lim\limits_{x \to -\infty}\frac{+\infty*-\infty}{-\infty}=-\infty$$
----- 
$$f(x)=0$$
$$\lim\limits_{x \to 0^+}f(x)=\lim\limits_{x \to 0^+}\cos(x)=1$$
$$\lim\limits_{x \to 0^{+}}\neq f(x)$$
-----
$$f(x)=\frac{x^3+2x^2+x}{x^3-x^2-2x}=\frac{(x)(x^2+2x+1)}{(x)(x^2-x-2)}=\frac{(x+1)(x+1)}{(x-2)(x+1)}=\frac{(x+1)}{(x-2)}$$
$$\lim\limits_{x \to 2^+}\frac{(x+1)}{(z-2)}=\lim\limits_{x \to 2^+}\frac{3}{\text{small}}=\infty$$
$$\lim\limits_{x \to 2^-}\frac{(x+1)}{(z-2)}=\lim\limits_{x \to -}\frac{3}{\text{-small}}=-\infty$$
---
$$g'(x)=\lim\limits_{h \to 0}\frac{\sqrt{x+h-1}-\sqrt{x-1}}{h}$$
$$\lim\limits_{h \to 0}\frac{(\sqrt{x+h-1}-\sqrt{x-1})}{h}*\frac{(\sqrt{x+h-1}+\sqrt{x-1})}{(h)(\sqrt{x+h-1}+\sqrt{x-1})}$$
$$\lim\limits_{h \to 0}\frac{x+h+1-x-1}{(h)(\sqrt{x+h-1}+\sqrt{x-1})}$$
$$\frac{1}{\sqrt{x-1}+\sqrt{x-1}}=\frac{1}{2\sqrt{x-1}}$$
$$\frac{1}{2\sqrt{1}}=\frac{1}{2}=g'(2)$$
---
$$y-1=\frac{1}{2}(x-2)$$
$$y=\frac{1}{2}x$$
---
$$\lim\limits_{h \to 0}\frac{\frac{1}{3x+h-1}-\frac{1}{3x-1}}{h}$$
$$\lim\limits_{h \to 0}\frac{\frac{(1)(3x-1)}{(3x+h-1)(3x-1)}-\frac{1(3x+h-1)}{(3x-1)(3x+h-1)}}{h}$$
$$\lim\limits_{h \to 0}\frac{\frac{3x-1-3x-h+1}{9x^2-3x+3xh-h-3x+1}}{h}=\lim\limits_{h \to 0}\frac{-1}{9x^2-6x+3xh-h}$$
$$f'(x) =\frac{-1}{9x^2-6x}=\frac{-1}{(3x)(3x-2)}$$
$$f'(1)=\frac{-1}{(3)(3-2)}=-\frac{1}{3}$$
---
$$y - \frac{1}{2}=-\frac{1}{3}(x-1)$$
$$y = - \frac{1}{3}x+ \frac{5}{6}$$
---
$$\lim\limits_{h \to 0}\frac{4(x+h)^2+2(x+h)+1-(4x^2+2x+1)}{h}$$
$$\lim\limits_{h \to 0}\frac{4x^2+8xh+4h^2+2x+2h+1-4x^2-2x-1}{h}$$
$$\lim\limits_{h \to 0}\frac{8xh+4h^2+2h}{h}$$
$$\lim\limits_{h \to 0}8x+4h+2$$
$$f'(x)=8x+2$$
---
$$f'(x)=-10$$
$$-10=8x+2$$
$$-12=8x$$
$$x= \frac{-12}{8}=-1.5$$