#notes #math111 #math #calc



## Chain Rule Objectives
- State the chain rule: $$(f(g(x)))'=f'(g(x))*g'(x)$$
- Apply the chain rule to compute derivatives
- Apply for powers to find derivatives, if $n$ is any non-zero real number, then $$\frac{d}{dx}((g(x))^{n})=n(g(x))^{n-1}g'(x)$$
- Chain rule tells us how to differentiate a "composition" of functions
- So let's do an example
### ex
$h'(x)$ for $h(x)=(3x^{7}+1)^{2}$

$f'(x) =6x^{7}+2$
$g'(x)=21x^{6}$
$f'(x)*g'(x)=(6x^{7}+2)(21x^6)$
$h'(x)=126x^{13}+42x^{6}$

## Generalization Calls
- So, chain rule is quirky, and we can differentiate whatever the hell we want using the old rules

### Chain rule for powers
$$\frac{d}{dx}[(g(x))^{n}]=n(g(x))^{n-1}g'(x)$$
### Chain rule for exponentials
$$\frac{d}{dx}[e^{g(x)}]=e^{g(x)}*g'(x)$$
## Examples (but again)
### Let $y = \sqrt{x^4-7x}$

$y'=\frac{1}{2}(x^4-7x)^{\frac{-1}{2}}*(x^4-7x)''$
$y'=\frac{1}{2}(x^{4}-7x)^{\frac{-1}{2}}*(4x^3-7)$

### Let $f(x) = 3e^{4\sqrt{x}}$
$f'(x)=3e^{4\sqrt{x}}*2x^{\frac{-1}{2}}$

### Use the chain rule to find $(e^{ax})'$
- where A is just some number
- $f'(x) = e^{ax}*a$
- 