#notes #math111 #math #calc

## Quotient Rule
$$\frac{d}{dx}(\frac{f(x)}{g(x)})=\frac{g(x)f'(x)-f(x)g'(x)}{(g(x))^2}$$
shorter version
$$(\frac{f}{g})'=\frac{g*f'-f*g'}{g^{2}}$$
$$\frac{Hi}{Lo}=\frac{Lo*DHi-Hi*DLo}{Lo^2}$$
- Why does the quotient rule work?
- We could prove it using the limit definition of the deriative
	- oooooooooooooor we can wait until we know the chain rule
		- you don't even really need the quotient rule, but the chain rule can do it instead (or product, combined shenanigans of both)

### Ex
let $y = \frac{x^4+3x}{10-x}$
$$lo'=0-1$$
$$hi'=4x^3+3$$
$$\frac{(10-x)(4x^3+3)-(x^4+3x)(-1)}{(10-x)^2}$$
you coooould simplify slightly $$\frac{dy}{dx}\ \ \frac{(10-x)(4x^3+3)+(x^4+3x)}{(10-x)^2}$$

we aa

---
Find $f'(x)$ of $f(x)=\frac{x^{2}}{4}$


quotient time
$lo' =0$
$hi'=2x$
$$\frac{(4)(2x)-(x^2)(0)}{4^2}=\frac{(4)(2x)}{4^2}=\frac{2x}{4}=\frac{x}{2}$$
other way time
$$0.25*x^2=0.5x=\frac{x}{2}$$

## Derivatives of Trig Functions

$\frac{d}{dx}\sin(x)=\cos(x)$
$\frac{d}{dx}\cos(x)=-\sin(x)$

They're the basic ones, you can plug everything else in

$\frac{d}{dx}\tan(x)=\sec^2x$
$\frac{d}{dx}(\sec(x))=\sec x \tan x$
$\frac{d}{dx} cot(x) = -\csc^2x$
$\frac{d}{dx}\csc x = -\csc x \cot x$

Memory tip: sst

secx secx tanx
cscx cscx cotx


secx->  secx <- tanx

cscx->  -cscx <- cotx

---

Show that $\frac{d}{dx}(\tan x) = sec^2x$
$$\frac{\sin}{\cos}'=\frac{(\cos)(\sin x)' - (\sin x)(\cos x)'}{\cos^2x}=\frac{\cos x * \cos x-\sin x(-\sin x)}{\cos^{2}x}=\frac{1}{\cos ^2x}=\sec^2x$$

