#notes #math213 #math #calc


### Double Integrals over General Regions
- So like, not just rectangular regions

#### Type 1: Vertical Regions
- Rectangles here are going to be parallel to the y axis, x bounds are going to be from $a,b$ but y is going to vary between your functions, $h(x)$ and $g(x)$
- Type 1 will have one top function and one bottom function for the entire region 
- $R := \{(x,y) \mid a \leq x \leq b, g(x) \leq y \leq h(x)\}$
$$V = \int_{a}^{b}\int_{g(x)}^{h(x) }f(x,y) dydx$$
- This is *y* first, just writing that for posterity

#### Type 2: Horizontal 
- Rectangles are going to be parallel to the y axis (that shit crazy. who could've seen this coming.
- Guess what? $R:= \{(x,y) \mid g(y) \leq x \leq h(y), c \leq y \leq d\}$
$$\int_{c}^{d}\int_{g(x)}^{h(x)}f(x,y)dxdy $$
- Fun Note: there will not be functions on the outer bound <sub>in calc 3...</sub>

### Exampling Time
- Let $R$ be the region in the plane between $y=2x,y=6x,$ and the y axis. Compute $\iint_{R}(x-2y)dA$
![[double integral first sketch]]
- Quick bound solving, $6-x=2x$ at $x=2$
- This is going to be a TYPE ONE, with vertical bounds

$$\int_{0}^{2} \int_{2x}^{6-x} (x-2y)dydx$$
- And now we integrate

$$\int_{0}^{2}( xy -y^{2}\Big|_{2x}^{6-x})dx$$
$$\int_{0}^{2}(x(6-x) - (6-x)^{2} )- (x(2x )- (2x)^{2})dx$$
$$\int_{0}^{2}(6x-x^{2}-36 +12x -x^{2}-2x^{2}+4x^{2})dx $$
$$\int_{0}^{2}(18x-36)dx$$
$$9x^{2}- 36x \Big|_{0}^{2}= 36 -72 = -36$$
### Example but again (there was a brief interlude regarding the chopping of fingers before this)
- Compute $\iint_{R} xy \ dA$ bounded by $y=x-1$ and $y^{2}= 2x+6$
- $x= \frac{1}{2}y^{2}-3$ 
![[case 2 double integral thing]]
$$\int_{-2}^{4}\int_{\frac{1}{2}y^{2}-3 }^{y+1 }xy \ dxdy$$
$y+1 = \frac{1}{2}y^{2}-3$
$\frac{1}{2}y^{2}-y -4 = 0$
$y^{2} -2y - 8 = (y+2)(y-4)$

$$\int_{-2}^{4} \frac{x^{2}y}{2} \Big|_{\frac{1}{2}y^{2}-3}^{y+1} $$
$$\frac{1}{2}\int_{2}^{4}\left((y+1)^{2}y - \left(\frac{1}{2}y^{2}-3\right)^{2}y\right)dy$$
$$= \frac{1}{2}\int_{-2}^{4}y(y+1)^{2}dy - \frac{1}{2}\int _{-2}^{4} (\frac{1}{2}y^{2}-3)^{2}y dy$$
- Let u = y+1, du = dy, y = u-1

$$\frac{1}{2}\int(u-1)u^{2}du= \frac{1}{2}( \frac{u^{4}}{4}- \frac{u^{3}}{3})$$
$$\frac{1}{2}( \frac{(y+1)^{4}}{4}- \frac{(y+1)^{3}}{3}\Big|_{-2}^{4})$$
$$\frac{1}{2}\left(\left(\frac{5^{4}}{4}- \frac{5^{3}}{3}\right)- (\frac{1}{4}+ \frac{1}{3})\right)$$
$$- \frac{1}{2}\int_{-2}^{4} (\frac{1}{2}y^{2}-3)^{2}y  \ dy$$
- W = $\frac{1}{2}y^{2}-3$, $dw=ydy$

$$\frac{-1}{2}\int w^{2}dw$$
$$- \frac{1}{2} \frac{w^{3}}{3}$$
$$\frac{-1}{6}\int \left(\frac{1}{2}y^{2}-3\right)^{3} \Big|_{-2}^{4}$$
$$- \frac{1}{6}(5^{3}- (-1)^{3})$$
$$\iint = \frac{1}{2}( \frac{5^{4}}{4}- \frac{5^{3}}{3})- \frac{1}{4}- \frac{1}{3} -  \frac{1}{6}(5^{3}+1)$$
$$\iint = \frac{5^{4}}{8}+ \frac{5^{3}}{6}- \frac{1}{8}- \frac{1}{6}- \frac{5^{3}}{6}- \frac{1}{6}$$
$$\iint = \frac{5^{4}-1}{8}- \frac{2(5^{3}+1)}{6}$$
$$\iint = \frac{5^{4}-1}{8}- \frac{5^{3}+1}{3}= 78 - 42 = 36$$
