#notes #math213 #math #calc

## moving around to three variable changes of variables
- Where T, our transformation 
	- $x=g(u,v,w)$
	- $y=h(u,v,w)$
	- $z=p(u,v,w)$
- maps a bounded region $S$ onto a region $D$. Assume $T$ is a one-to-one and $g,h,\&\ p$ have continuous partial, then
$$\iiint_{D}f(x,y,z)dV = \iiint_{S}f(g,h,p) \mid J(u,v,w) \mid dV$$
When $J(u,v,w)$ is given by $$\begin{matrix}\frac{\partial x}{\partial u} & \frac{\partial x}{\partial v} & \frac{\partial x}{\partial w} \\ \frac{\partial y}{\partial u} \ & \frac{\partial y}{\partial v} & \frac{\partial y}{\partial w} \\ \frac{\partial z}{\partial u} & \frac{\partial z}{\partial v} &\frac{\partial z}{\partial w}\end{matrix}$$
			- i hate that
- Verify that $dV = \rho^{2}\sin\phi\ d\rho \ d\phi \ d\theta$ when transforming from rectangular to spherical
- So our transformation, $T$, ends up looking something like
	- $x= \rho\sin\phi\cos\theta$
	- $y=\rho\sin\phi\cos\phi$
	- $\theta = \rho\cos\phi$ 

$$\begin{matrix}\sin\phi\cos\theta & \rho\cos\phi\cos\theta & -\rho\sin\phi\sin\theta \\ \sin\phi\sin\theta & \rho\cos\phi\sin\theta & \rho\sin\phi\cos\theta \\ \cos\phi & -\rho\sin\phi & 0\end{matrix}$$
$$= \sin\phi\cos\theta(\rho^{2}\sin^{2}\phi\cos\theta) - \rho\cos\phi\sin\theta(\rho\sin\phi\cos\phi\cos\theta) $$
$$-\rho\sin\phi\sin\theta( \sin\phi\sin\theta(-\rho\sin\phi) - \rho\cos\phi\sin\theta\cos\phi )$$
$$\rho^{2}\sin^{3}\phi \cos^{2}\theta + \rho^{2}\sin\phi\cos\phi\cos^{2}\theta + \rho^{2}\sin^{3}\phi \sin^{2}\theta + \rho^{2}\sin\phi\cos^{2}\phi\sin^{2}\theta$$
$$\rho^{2}\sin^{3}\phi(1) + \rho^{2}\sin\phi\cos^{2}\phi(1) = \rho^{2}\sin\phi (\sin^{2}\phi + \cos^{2}\phi)= \rho^{2}\sin\phi$$
### try one!
- Evaluate $\iiint_{D}xz,$ where $D$ is bounded by $y=x,y=x+2,z=x,z=x+3,z=0,z=4$ 
	- Oh hey, $y=x$ and $y=x+2$ are parallel planes (using $y-x$)
		- Oh hey hey, $z=x$ and $z=x+3$ are parallel (using $z-x$)
			- Oh hey hey hey, $z=0$ and $z=4$ are parallel
	- This is what we in the business call a "parallelepiped"
	- We can say that $u=y-x$, which then bounds it between 0 and 2
	- $v=z-x$, which then bounds us between 0 and 3.
	- $w=z$, bounded between 0 and 4
![[flippy the parallelepiped]]
- I've done worse sketches.

- Ok, now to do our actual integral.

$$\iiint_{D}xz dV= \int_{0}^{4}\int_{0}^{3}\int_{0}^{2}f(u,v,w) \mid J(u,v,w) | dudvdw$$
$$\int_{0}^{4}\int_{0}^{3}\int_{0}^{2}w(w-v) \mid J(u,v,w) | dudvdw$$
$$x=z-v, x=w-v$$
$$y=u+w-v$$
$$z=w$$
$$\det(\begin{matrix}0 & -1 & 1 \\ 1 & -1 & 1 \\ 0 & 0 & 1 \end{matrix}) = (0)-(-1)(1-0)+1(0)= 1$$
$$\int_{0}^{4}\int_{0}^{3}\int_{0}^{2}(w-v)w (1) dudvdw$$
$$2 \int_{0}^{4}\int_{0}^{3}(w^{2}-wv)dvdu$$
$$2\int_{0}^{4}(3w^{2}- \frac{9}{2}w)dW$$
$$2 (w^{3}- \frac{9}{4}w^{2}\Big|_{0}^{4})= 2(64 - 36)=56$$


---

Use the transformation
$$u=x+y$$
$$v=2x-y$$




$$y=2x-v$$
$$x=u-y$$
$$x=u-2x+v$$
$$3x=u+v$$
$$x = \frac{u+v}{3}$$
$$y = \frac{2(u+v)}{3}-v$$
$$y= \frac{2}{3}u - \frac{1}{3}v$$

$$\frac{2}{3}u - \frac{1}{3}v = - \frac{1}{3}u - \frac{1}{3}v$$
$$y=-x \to u=0$$
$$\frac{2}{3}u - \frac{1}{3}v = 2 - \frac{1}{3}u - \frac{1}{3}$$
$$y=2-x \to u = 2$$
$$\frac{2}{3}u - \frac{1}{3}v = 2 ( \frac{1}{3}u + \frac{1}{3}v)$$
$$0 \leq u \leq 2$$
$$-1 \leq v \leq 0$$
