#notes #math111 #math #calc

- Quick warning
	- Power rule is only good for $x$ to a power 
- product and quotient rules are a bit of a pain - remember that you can do algebra to get around doing them

Other fun fact
$$\frac{d}{dx}(e^{x)} = e^x$$
- There's some limit bs as to why, I'm half tempted to do the fanangling 

## okie dokie time for the real notes

#### Product Rule
$$\frac{d}{dx}(f(x)*g(x)) = f(x)g'(x) + g(x)f'(x)$$
Shorthand $$(fg)' = fg' + gf' $$

it is definitely NOT $$(fg)' \neq f'g'$$
##### Example: Find $h'(x)$ = $h(x) = 6x^{3} (2x^{2} -1 )$
- $f'(x) = 18x^{2}$
- $g'(x) = 4x$
- $h'(x) = (6x^{3})(4x) + (2x^2-1)(18x^2)$
- $h'(x)=60x^4-18x^2$
##### ex (again) Find $f'(x) = 2x^2e^x$
$g'(x)=4x$
$h'(x)=e^x$
$f'(x)=(4x)(e^x)+(2x^2)(e^x)$
$f'(x)=(e^x)(4x+2x^2)$

##### ex(three) Find $h'(x)(x^2+1)(3x^{-5} +x^{-1})$
$f'(x)=2x$
$g'(x)=-15x^{-6}-x^{-2}$
$h'(x)=(2x)(3x^{-5} + x^{-1}) + (x^{2}+1)(15x^{-6} - x^{-2})$
$h'(x)=6x^{-4}+2x + 15x^{-4}-1+15x^{-6}-x^{-2}$

## Why does the product rule work?
# Because Deb said so.
