#notes #math111 #math #calc


## we did some matching stuff
- had the epiphany about degrees of functions, that's so much fun
## Notion aside
$f'(x)=\frac{dy}{dx}$
$\frac{dy}{dx}$ is Leibniz notation, and we tend to use it as an operator
$(10)'$ means take the derivative of what's inside the parenthesis
# Alright time to learn shortcuts 

### Constant Rule
- If $f(x)=c$ then $f'(x)=0$
- If it's just a constant, then the slope of it 0 everywhere, wow, awesome

### Power Rule
- If $f(x)=x^n$  then $f'(x)=nx^{n-1}$
- So if it's just $f(x)=x$, then it comes out that $f'(x)=1$ (neat)
- $\frac{d}{dx}(x^{10})=10x^9$
- Remember that $\frac{1}{x^{2}}$ is the same thing as $x^{-2}$ 
- So the derivative of $\frac{1}{x^{2}}$ is $-2x^{-3}$

### Constant Multiple Rule
$$\frac{d}{dx}(cf(x))=cf'(x)$$
So the derivative of $10x^{-1}=10*(-1)x^{-2}$ 

### Sum (and Difference) Rule
$$\frac{d}{dx}(f(x)+g(x))=(f'(x)=g'(x))$$
Differentiating two different functions that are being added(or subtracted) ? Eh, just do em independently and then stick em together

Strictly speaking, this is following limit rules; A limit of a sum = the sum of the limits

### Example
Find $f'(x)$ for $6 \sqrt{x} +\frac{x^4}{2}+\frac{8}{x^11}+3x$

We gotta do some rewriting

$$f(x) = 6*x^{\frac{1}{2}}+ \frac{1}{2}x^{4} + 8x^{-11}+3x$$
So let's get derivin'
$$3x^{-0.5} + 2x^{3}-88x^{-12}+3$$
