#notes #math225 #math 
![[MATH225 - 2025-03-28 2025-03-28 13.01.59.excalidraw]]
- Quick circuit.

$$
\overbrace{ \epsilon }^{ Voltage }=\overbrace{ R }^{ \text{Resistance} } \frac{dq}{dt}+\frac{1}{\underbrace{ c }_{ \text{Capacitance} }}\overbrace{ q }^{ \text{Charge} }
$$
- We can solve this ODE relatively normally, and we end up with
$$
q(t)=c\epsilon(1-e^{-t/RC})
$$
- Let's suppose we have the switch as closed, and then we open it and turn it off. (ie, heaviside step function shenanigans)

So then

$$
\epsilon=1-u(t-t_{c})
$$
- We can solve this ode with $\mathcal{L}\{\}$ tranasform if we let R=1 megaohm, and C = 1 microfarad, and RC = 1 sec
$$
\frac{dq}{dt}+\frac{1}{RC}q=\frac{1}{R}[1-u(t-tc)]
$$
- Now for the actual Laplace step now that we've replaced everything
$$
Y(s+1)= \frac{1e-6}{s}[1-e^{-st_{c}}]
$$
- This is using $\mathcal{L}\{q\}=Y$
$$
q(t)=1e^{-6}[1-e^{-t}-u(t-t_{c})+u(t-t_{c})e^{-(t-t_{c})}]
$$
---

### "The Last Possible Topic that can be on the exam"
- ![[MATH225 - 2025-03-28 2025-03-28 13.20.11.excalidraw]]
- This is called a "Unity Impulse," because $\int_{-\infty}^{\infty}f(t)dt=1$
- Ok make this thing comically sharp. Probably d/dx sharp if I were to guess.
	- Either way, you make it sharper, and your integrals are always still one.

- In order to go infinitesimally small, we need a new function
##### Dirac Delta Function ($\delta$)
- Is, strictly speaking, the limit of that other shenanigans.
$$
\delta(x)=0 \ \ \ \text{if} \ \neq 0
$$
- At $x=0$, it's an infinitesimally wide spark.

$$
\int_{-\infty}^{\infty}\delta(x)dx=1
$$
- (Still a unity impulse)
- Amusing aside:
	- Dirac didn't actually prove this, he just started using it and its properties
$$
\int_{-\infty}^{\infty}f(x)\delta(x-a)dx=f(a)
$$
- We use $\delta$-fn to represent a sharp impulse
$$
\mathcal{L}\{\delta(t-t_{0})\}=e^{-st_{0}}
$$
---
##### Example
$$
\underbrace{ y''+\omega_{0}^{2}y }_{ \text{Homogeneous for undamped oscillator} }=\overbrace{ \delta(t-t_{0}) }^{ \text{Sharp impulse} }
$$
$$
y(0)=y'(0)=0
$$

$$
s^{2}Y-sy(0)-y'(0)+\omega_{0}^{2}Y=e^{-st_{0}}
$$
$$
Y=\frac{e^{-st_{0}}}{s^{2}+\omega_{0}^{2}}
$$
$$
\mathcal{L}^{-1}\left\{ \frac{e^{-st_{0}}}{s^{2}+\omega_{0}^{2}} \right\}
$$
- Pop our good old friend friend formula 5 in.
	- $a=t_{0}$, $F(s)=\frac{1}{s^{2}+\omega_{0}^{2}}$
	- use formula 14 for that transform there on F(s)
$$
\mathcal{L}^{-1}\left\{ \frac{e^{-st_{0}}}{s^{2}+\omega_{0}^{2}} \right\}=u(t-t_{0}) * \frac{1}{\omega_{0}} * \sin(\omega_{0}(t-t_{0}))
$$
