#notes #math225 #math 

## Previously On
- We were dealing with complex numbers ($z=a+bi$), the conjugates of a complex number being $\bar{z}=a-bi$, the modulus of a complex number being $|z|=\sqrt{ z*\bar{z} }$ 
- We can also write a complex number as the equivalent from $z=re^{i\theta}$
	- Note that this way also takes two constants to define, they're just $r$ and $\theta$ instead of $a,b$
	- $z=re^{i\theta}=r\cos\theta+ir\sin\theta$
	- $\bar{z}=r\cos\theta-ir\sin\theta=re^{-i\theta}$
		- If you have $re^{-i\theta}=re^{i(-\theta)}=r(\cos(-\theta)+i\sin(-\theta))=r(\cos\theta-i\sin(\theta))$
	- So if we use $z=re^{i\theta}$, we've just proven that its conjugate, $|z|=re^{-i\theta}$
- Fun fact, you can represent a complex number as a vector in two dimensions (isn't it neat how it also takes two number inputs, just like a 2-d vector)
![[Real Imaginary graphing]]
- By and large differential equations isn't a vector analysis class, so we don't really care too much.
	- However, this shows up all the damn time in all kinds of other situations.
#### Euler's Formula
$$
e^{i\theta}=\cos\theta+i\sin\theta
$$
$$
e^{-i\theta}=\cos\theta-i\sin\theta
$$
- We do this through the fact that $\cos(-\theta)=\cos(\theta)$ and $\sin(-\theta)=-\sin(\theta)$
$$
z\cos\theta=e^{i\theta}+e^{-i\theta}
$$
$$
\cos\theta = \frac{e^{i\theta}+e^{-i\theta}}{z}
$$
$$
\sin\theta=\frac{1}{2i}[e^{i\theta}-e^{-i\theta}]
$$
---
#### Quick Aside - Roots of $i$
$$
e^{i \frac{\pi}{2}}= \cos\left( \frac{\pi}{2} \right)+i\sin\left( \frac{\pi}{2} \right)=0+i=i
$$
So $\sqrt{ i }=i^{1/2 }=(e^{i \ \pi/2})^{1/2}=e^{i \ \pi/4}$
Which is then $\cos\left( \frac{\pi}{4} \right)+i\sin\left( \frac{\pi}{4} \right)$
- To get the cube root of $i$, you end up with $\frac{\pi}{6}$, and have to do the same kind of calculations.

---

## How to Solve Homogeneous Second Order Differential Equations with Constant Coefficients 
$$
\text{General form of: }ay''+by'+cy=0
$$
- $a,b,c$ are all just numbers, not functions or any such nonsense.
- We're going to be here a while.
	- Pops up all the time in Newton's Second Law (with acceleration/velocity/position), EE type shit with Kirchoff's Law, etc, etc
- At some point<sub> by which I mean yesterday</sub>, we wrote the equation $y''-y'-12y=0$
	- And we asserted that $e^{-3x}$ and $e^{4x}$ are solutions, which we proved and got to work, and ended up with the general solution $y=c_{1}e^{-3x}+c_{2}e^{4x}$
- We investigate whether solutions can always be written as $e^{mx}$
	- If we assume the solution is $y=e^{mx}$, then $y'=me^{mx}$, and $y''=m^{2}e^{mx}$
	- Then we have $em^{2}e^{mx}+bme^{mx}+ce^{mx}=0$
		- Factor a smidge, you get $e^{mx}(am^{2}+bm+c)=0$
			- $e^{mx}$ is never zero, so you can divide by it, so $am^{2}+bm+c=0$
			- This neat little equation we've made is called the auxiliary equation, and occasionally the characteristic equation
	- We then solve for $m$, then the solution to the DE is $e^{mx}$
- The characteristic equation can have
	1. Two real roots
	2. Repeated real roots
	3. Two complex conjugate roots
----

### Alright, enough talk. Example time.
$$
y''-y'-6y=0
$$
- That there is our differential equation.
- First up, write the characteristic equation, which will be $m^{2}-m-6=0$
	- $(m-3)(m+2)=0$
	- $m=3$ and $m=-2$ are the roots of this equation
	- Which sure look like two real, not repeated roots
- So the solution is $$
 y=c_{1}e^{3x}+c_{2}e^{-2x}
$$
---
$$
y''-10y'+25y=0
$$
- Characteristic equation becomes $m^{2}-10m+25=0$, or $(m-5)^{2}=0$, which is $m=5$ as a repeated real root
- One solution is $e^{5x}$, however we need another linearly independent solution because of how second order works
- The second solution, however, is actually just $xe^{5x}$, so you're really just slapping an $x$ on.
$$
y=xe^{5x},y'=5xe^{5x}+e^{5x}, y''=25xe^{5x}+5e^{5x}+5e^{5x}
$$
$$
25xe^{5x}+10e^{5x}-50xe^{5x}-10e^{5x}+25xe^{5x}=0
$$
- That's a lotta $e^{5x}$