#notes #math225 #math 


## getting muc-y with it
$$y' + ay = f(t)$$

- this only works for a certain set of functions for $f(t)$
	- this can be a polynomial ($f(t)=t^{2}+1$ is perfectly polynomial, for instance) 
	- exponential ($f(t)=2e^{t}$, for instance)
	- can be sine or cosine
	- Combinations of any of those

##### General Solution
$$y=y_{c}+y_{p}$$
- The $y_{c}$ is the complementary, or homogenous solution
- The $y_{p}$ is the particular solution 
##### Homogenous equation
- Has a right hand side = 0 so $$y'+ay=0$$
- You can almost certainly separation of variables that, so $$\ln(y)-at +c_{1}$$$$y = c_{1}e^{-at}$$
- Which means the original form is going to be $$y= c_{1}e^{-at}+y_{p}$$
##### The particular part
- New problem: finding $y_{p}$
	- Solution: just fucking guess.
$$2y' + 6y = e^{-t}$$
$$-> y' + 3y = \frac{1}{2} e^{-t}$$
- We need some $y_{p}$ that produces $\frac{1}{2}e^{-t}$ when plugged in to the left hand side. Given that the only damn thing that derives itself into an exponential is an exponential, we're just going to guess $$y_{p}= Ae^{-t}$$
- The A is the undetermined coefficient in question (bum bum buuuum)
	- If we're calling that $y_{p,}$ then $y_{p}'=-Ae^{-t}$
$$2Ae^{-t}+6Ae^{-t}=e^{-t} -> 4Ae^{-t}=e^{-t}$$
- Which just gives you $4A=1$, so $A = \frac{1}{4}$ 
- Our overall answer is then smacking them together
$$y=c_{1}e^{-3t}+ \frac{1}{4}e^{-t}$$

| $f(t)$        | Guess                                           |
| ------------- | ----------------------------------------------- |
| $e^{2t}$      | $Ae^{2t}$                                       |
| $\sin(3t)$    | $A\sin(3t)+B\cos(3t)$                           |
| $\cos(3t)$    | $A\sin(3t)+B\cos(3t)$                           |
| $t^{3}$       | $At^{3}+Bt^{2}+Ct+D$                            |
| $t^{2}e^{t}$  | $(At^{2}+Bt+C)e^{-t}$                           |
| $t^2\sin(4t)$ | $(At^{2}+Bt+C)(\sin(4t))+(Dt^2+Et+F)(\cos(4t))$ |
| $e^{-t}+t$    | $Ae^{-t}+Bt+C$                                  |
|               |                                                 |
### example time

$$\frac{dy}{dx}-y = 1$$
- I mean, sure looks separable to me
$$\frac{dy}{y+1}=dx$$
$$\ln(y+1)=x+c$$
$$y+1=c_{1}e^{x}$$
$$y=c_{1}e^{x}-1$$
- I mean, y'know, when in Rome, sure looks integrating factor-able to me
$$\mu = e^{\int(-1)dx}=e^{-x}$$
$$(e^{-x}y)' =e^{-x}$$
$$e^{-x}y=-e^{-x}+c_{1}$$
$$y = \frac{c_{1}}{e^{-x}}-1$$
- I mean, y'know, when in Rome, sure looks muc-able to me.
$$y = y_{c}+ y_{p}$$
$$y_{c}= c_{1}e^{x}+y_{p}$$
- We're just going to guess that $y_{p}$ is a constant, since the right side is basically just a low order polynomial (also, $y_{p}' =0$)
	- lob that back in to our differential equation
		- $-A=1$, $A=-1$
$$y=c_{1}e^{x}-1$$
#### new example
$$y'-y=\cos(2x)$$
$$\frac{dy}{dx}-y = \cos(2x)$$
- That sure doesn't look separable, you coooould integrating factor, but then you'd have to (probably repeated) integration by parts, and.... we don't wanna
- So instead, muc!
$$y=y_{c}+ y_{p}$$
$$c_{1}e^{x}+y_{p}$$
- Oh hey, we have a cosine lying around, so we're going to guess those are hopping around
$$y_{p}= A\cos(2x)+B\sin(2x)$$
$$y_{p}' = -2A\sin(2x)+2B\cos(2x)$$
- Plug that back in to the original differential equation

$$-2A\sin(2x)+2B\cos(2x) + A\cos(2x)+B\sin(2x)=\cos(2x)$$
$$(-2A-B)(\sin(2x))=0$$
$$(2B-A)(\cos(2x))=\cos(2x)$$
$$2B-A=1$$
$$-2A-B=0$$
$$B=-2A$$
$$-4A-A=1$$
$$-5A=1, A = - \frac{1}{5}$$
$$B = \frac{2}{5}$$
- So, overall becomes
$$c_{1}e^{x}- \frac{1}{5}\cos(2x) + \frac{2}{5}\sin(2x)$$