#notes #math225 #math 
## when muc fails (or is at least weird)
- This is when the homogeneous solution includes our guess for $y_{p}$
$$y' +2y = 3e^{-2t}$$
$$y = y_{c}+y_{p}$$
- $y_{c}$ is the homogeneous solution, which solves 
$$y'+2y=0$$
- Which, in this case, is $y_{c}= c_{1}e^{-2t}$
- Our usual guess is $y_{p}=Ae^{-2t}$
	- uhhhhhhh, minor problem, it's looking an awful lot like we're going to get ourselves a zero if we keep barking down this tree
- In this case, we're just going to throw an extra $t$ in there, so our guess is going to become $y_{p}=Ate^{-2t}$

$$y_{p}= Ate^{-2t}$$
$$y_{p}' = -2Ate^{-2t}+Ae^{-2t}$$
- So we then lob back in to the original differential equation
$$-2Ate^{-2t}+Ae^{-2t}+2Ate^{-2t}=3e^{-2t}$$
- Group like powers of t
	- I mean, we can just divide fucking everything by $e^{-2t}$
$$-2At +A +2At = 3$$
$$A=3$$
- So then our general solution just becomes 

$$y =c_{1}e^{-2t} + 3te^{-2t}$$
- So just, as a rule of thumb, always check that your guess is not already included in the homogeneous solution.
	- If things go wrong around the solving for $A$ section, you probably forgot to check and should double back
### transience
- Sometimes, we might get solutions that look like $$y=c_{1}e^{-t}+\cos(t)$$
- $c_{1}e^{-t}$ is referred to as transient, since it does something we care about for a limited time (I love act 3 slay the spire)
- $\cos(t)$ is called the steady state, since it's what happens in the long term
- We'll eventually get back here with higher order equations

### other such fun things
$$\frac{dy}{dx}+ \frac{2}{x}y=x$$
$$x (\frac{dy}{dx})+ 2y = x^{2}$$
$$x(\frac{dy}{dx}-x)=-2y$$
- I swear this is separable, but, regardless, we use integrating factors
	- Did I do legal math up there? Is that separate? the dy/dx is perpetually a bit confusing to me 

$$e^{\int p (x)dx}=e^{\int \frac{2}{x}dx}=e^{2\ln(x)}=e^{\ln(x^{2})}=x^{2}$$

$$(x^{2}y)' = x^{3}, x^{2}y = \frac{x^{4}}{4}+c_{1}$$
$$y=\frac{x^{2}}{4}+ \frac{c_{1}}{x^{2}}$$
## now we get another one (substitution method)
- Applies to Bernoulli Equation(s)
$$\frac{dy}{dx}+ p(x)y = f(x)y^{n}$$
- We're going to use a substitution of $u=y^{1-n}$. This will produce a linear equation in $u$ 
	- This is, of note, only really relevant for $y\neq 0 \ \& \ y\neq 1$, since like, yeaaaah.
- $$x \frac{dy}{dx}+ y = \frac{1}{y^{2}}$$
- $$\frac{dy}{dx}+ \frac{1}{x}y = \frac{1}{x}* \frac{1}{y^{2}}$$
- This is now a Bernoulli equation with $n=-2$
- We let $u=y^1--2=y^{3}$, or $y = u^{\frac{1}{3}}$ 
$$\frac{dy}{dx}= \frac{dy}{du} \frac{du}{dx}$$
- You always end up having to do this funky conversion whenever you're doing a Bernoulli equation
$$\frac{dy}{du}= \frac{1}{3}u^{\frac{-2}{3}}$$
$$\frac{dy}{dx}= \frac{1}{3}u^{\frac{-2}{3}} \frac{du}{dx}$$
$$\frac{1}{3}u^{\frac{-2}{3}} \frac{du}{dx}+ \frac{1}{x}u^{\frac{1}{3}}= \frac{1}{x}u^{\frac{-2}{3}}$$
- Multiply by $3u^{2/3}$ to hopefully clear out a whole bunch of things
$$u' + \frac{3}{x}u + \frac{3}{x}$$
- We are, quite unfortunately, in a rut of having to do some integrating factors
$$u = e^{\int \frac{3}{x}dx }=x^{3}$$
$$\frac{du}{dx}+ \frac{3}{x}u = \frac{3}{x} \to (x^{3}u)' = 3x^{2}$$
$$x^{3}u = x^{3} +c_{1}$$
$$u = 1+ \frac{c_{1}x}{3}$$
buuut $u = y^{3}$
so $$y^{3} = 1 + \frac{c_{1}}{x^{3}}$$
- If you really want to make this explicit, you're going to have to cube root this entire thing, but like, that's a lotta work
$$\frac{du}{dx}+ \frac{3}{x}u = \frac{3}{x}$$
$$\frac{du}{dx}= \frac{3}{x}(1-u)$$
$$\frac{du}{1-u}= \frac{3}{x}dx$$
$$-\ln(1-u) = 3\ln(x)+c_{1}$$
- That's separation, presumably if you keep cooking you'll get somewhere reasonable

- And that's presumably it for linear equations, now we're going to get into physical models to actually use differential equations
- 