#notes #math225 #math 

$$
f(t) = \begin{cases}
t & 0\leq t\leq{2} \\
0 & t>2
\end{cases}
\implies f(t)=t-t*u(t-2)
$$
- Again, the whole reason we're doing this is to do Laplace transforms, sooo
$$
\mathcal{L}\{u(t-a)*f(t-a)\}=e^{-as}F(s)
$$
- That's nice, but the alternate form of 
$$
\mathcal{L}\{g(t)*u(t-a)\}=e^{-as}\mathcal{L}\{g(t+a)\}
$$
---
$$
\mathcal{L}\{u(t-2)*\sin(t-2)\}
$$
- This just looks like formula 5 with $a=2$ and $f(t)=\sin(t)$
- if $f(t)=\sin(t)$ then $F(s)=\frac{1}{s^{2}+1}$
---

$$
\mathcal{L}^{-1}\left\{ \frac{e^{-2s}}{s^{3}} \right\}
$$
- This sure looks like 5 with $a=2$ and $F(s)=\frac{1}{s^{3}}$
- 5:  $u(t-a)f(t-a)\stackrel{\mathcal{L}}{=}e^{-as}F(s)$
- If $F(s)=\frac{1}{s^{3}}$ then $f(t)$
- 9: $t^{n}\implies \frac{n!}{s^{n+1}}$ or $t^{2}\implies \frac{2!}{s^{3}}$

$$
u(t-2) * \frac{1}{2 }(t-2)^{2}
$$

----

$$
\mathcal{L}^{-1}\left\{ e^{-s} * \frac{1}{(s+3)^{2}} \right\}
$$
- This is, believe it or not, five again.
	- $a=1,F(s)=\frac{1}{(s+3)^{2}}$ 
$$
f(t)=\mathcal{L}^{-1}\left\{ \frac{1}{(s+3)^{2}} \right\}
$$
- We're going to pop formula sixteen in, which is that $t^{n}e^{at} \implies \frac{n!}{(s-a)^{n+1}}$
	- So therefore $te^{-3t}=\frac{1}{(s+3)^{2}}$
- Oookie dokies, so using 5 we then get
	- $u(t-1)*(t-)e^{-3(t-1)}$
---

![[MATH225 - 2025-03-26 2025-03-26 13.23.20.excalidraw]]
- If we want to find $\mathcal{L}\{f(t)\}$ of that, first we need to write out function out

$$
f(t)=\underbrace{ 2 }_{ 7 }-\underbrace{ 3u(t-2) }_{ 19 }+\underbrace{ u(t-3) }_{ 19 }
$$
---

$$
y'+y=f(t), \ \ y(0)=0
$$
$$
f(t)=\begin{cases}
0 & 0 \leq t \leq 1 \\
5 & t>1
\end{cases}
= 5u(t-1)
$$
- Get Laplace-y with it
$$
\overbrace{ sY-y(0) }^{ F{1} }+Y= \overbrace{ \frac{5*e^{-s}}{s} }^{ F 19 }
$$
$$
Y=\frac{5e^{-s}}{s(s+1)}
$$
- That's an answer... which is unfortunately stuck in the wrong domain. Let's go transform it back
$$
y(t)=\mathcal{L}^{-1}\left\{ \frac{5e^{-s}}{s(s+1)} \right\}
$$
$$
\frac{5}{s(s+1)}=\frac{A}{s}+\frac{B}{s+1}
$$
$$
As+A+B=5
$$
$$
A=5, B=-5
$$

$$
\mathcal{L}^{-1}\left\{ e^{-s}\left[ \frac{5}{s}-\frac{5}{s+1} \right] \right\}
$$
- We pop equation 5 back in
$$
\mathcal{L}^{-1}\left\{ \frac{5e^{-s}}{s} \right\}=5u(t-1)
$$
- Believe it or not, we're using equation 5 again with a=1 and $F(s)=\frac{1}{s+1}$ which we then transform with 12 into $e^{-t}$
$$
\mathcal{L}^{-1}\left\{ -\frac{5e^{-s}}{s+1} \right\}=-5u(t-1)e^{-(t-1)}
$$
- So our final answer becomes 
$$
5u(t-1)-5u(t-1)e^{-(t-1)}
$$
---

$$
y''+16y=0
$$