#notes #math225 #math 


## More Examples and Review

$$
\mathcal{L}\{f(t)\}=\frac{2}{s^{2}}
$$
- What is the laplace transform of.
$$
\mathcal{L}\{e^{2t}f(t)\}
$$
$$
f(t)=2t
$$
$$
\mathcal{L}\{2te^{2t}\}= 2 * \left( \frac{1}{(2-a)^{}} \right)
$$
---
Change the problem!

$$
\mathcal{L}\{f(t)\}=\frac{2}{s^{3}}
$$
$$
t^2=f(t)
$$
$$
\mathcal{L}\{t^{2}e^{2t}\}=\frac{2}{(s-2)^{3}}
$$
----
- Formula six is NOT multiplication
$$
f(t)*g(t)=\int_{0}^{t}f(\tau)g(t-\tau)d\tau
$$
- That $*$ is a convolution, NOT NOT NOT multiplication
----


$$
y''+4y'+8y=0
$$
$$
y(0)=y'(0)=0
$$
- The solution here is just $y=0$ since it's a physical system sitting at equilibrium as all of nothing happens.
$$
s^{2}Y-sy(0)-y'(0) + 4 ( sY-y(0)) + 8Y=0
$$
$$
s^{2}Y-0-0+4sY+8Y
$$
$$
Y(s^{2}+4s+8)=0
$$
$$
Y=0
$$
$$
\mathcal{L}^{-1}\{Y\}=0
$$
---------
- If we wiggle the initial conditions a bit
$$
y(0)=0,y'(0)=2
$$
- Keep the transform from earlier
$$
s^{2}Y-sy(0)-2 + 4 ( sY-y(0)) + 8Y=0
$$
$$
s^{2}Y-2+4(sY)+8Y
$$
$$
Y(s^{2}+4s+8)+2 = 0
$$
$$
Y=-\frac{2}{s^{2}+4s+8}
$$
$$
\mathcal{L}^{-1}\{Y\}=\mathcal{L}^{-1}\left\{ \frac{2}{s^{2}+4s+8} \right\}
$$
- If we go and complete the square here (which I'm not great at), we end up with
$$
\mathcal{L}^{-1}\left\{ \frac{2}{s^{2}+4s+4+4} \right\}
$$
$$
\mathcal{L}^{-1}\left\{ \frac{2}{(s+2)^{2}+4} \right\}
$$
- This is giving formula 18.
$$
\frac{2}{(s--2)^{2}+2^{2}}, a=-2, k=2
$$
$$
\mathcal{L}^{-1}\left\{ \frac{2}{(s+2)^{2}+4} \right\}=e^{-2t}\sin(2t)
$$
- You could also characteristic equation this, you get 
$$
r=-\frac{4\pm \sqrt{ 16-32 }}{2}=-2\pm_{2}i
$$
$$
f(t)=c_{1}e^{-2t}\cos(2t)+c_{2}e^{-2t}\sin(2t)
$$
- Which gives you $c_{1}=0$ and $c_{2}=1$
- There might be a situation or two where you're forced to do characteristic, but the general vibe is do whatever.
---

$$
\mathcal{L}^{-1}\left\{ \frac{1}{(s+2)^{2}} \right\}=te^{-2t}
$$
---
### Differential equation with piecewise driving force
- We worked this one in class, so you get my class notes thrown in of an actual explanation. Merry Christmas?
$$
y''+4y=f(t)
$$
$$
f(t) = \begin{cases}
0  & 0 \leq t \leq 4 \\
10e^{t-4} & t > 4
\end{cases}
$$
- We're going to write $f(t)$ in terms of Heaviside shenanigans
$$
f(t) = 10e^{t-4}u(t-4)
$$
- We're hitting this one with a transform
$$
s^{2}Y-sy(0)-y'(0)+4\left( Y \right)=\frac{10e^{-4s}}{s-1}
$$
$$
Y=\frac{10e^{-4s}}{(s^{2}+4)(s-1)}
$$
- uh, this smells awfully of partial fractions
$$
\frac{10}{(s^{2}+4)(s-1)}=\frac{As+B}{s^{2}+4}+\frac{C}{s-1}
$$
$$
(As+B)(s-1)+C(s^{2}+4)=10
$$
$$
As^{2}-As+Bs-B+Cs^{2}+4C=10
$$
$$
A+C=0
$$
$$
B-A=0
$$
$$
-B+4C=10
$$
$$
\frac{10}{(s-1)(s^{2}+4)}=-\frac{2(s+1)}{s^{2}+4}+\frac{2}{s-1}
$$
$$
\mathcal{L}^{-1}\{-\frac{2(s+1)}{s^{2}+4}+\frac{2}{s-1}\} = 2e^{t}-2(\cos(2t)+\sin(t)\cos(t))
$$
---
$$
f(t)= \begin{cases}
0 & t<3 \\
4 & t\geq 3
\end{cases}
$$
$$
2y''+4y'+4y=4u(t-3), \ \ \ y'(0)=y(0)=0
$$
 $$
2(s^{2}Y(s)-sy(0)-y'(0)) + 4 (2Y(s)-y(0))+4Y=\frac{e^{-4s}}{s}
$$
$$
2s^{2}Y(s)+8(Y(s))+4Y(s) = \frac{e^{-4s}}{s}
$$
$$
Y(2s^{2}+12)= \frac{e^{-4s}}{s}
$$
$$
Y=\frac{e^{-4s}}{s(2s^{2}+12)}
$$
$$
y(t)=u(t-4) \mathcal{L}^{-1}\left\{ \frac{1}{2s^{3}+12s} \right\}
$$
$$
\mathcal{L}^{-1}\left\{ \frac{1}{2s^{3}+12s} \right\}=\mathcal{L}^{-1}\left\{ \frac{1}{2s(s^{2}+6)} \right\}=\frac{1}{12}(1-\cos(\sqrt{ 6 }t))
$$
$$
y(t)=u(t-4)\left( \frac{1}{12} \right)(1-\cos(\sqrt{ 6 }t))
$$


