#notes #math112 #math #calc

$$f(x) = \sum\limits_{k=0}^{\infty}\frac{f^{(k)}(a)}{k!}(x-a)^{k}$$
Find Taylor series for different functions 

Starting with $f(x) = \frac{1}{x}$, centered at $x=3$


| $f^{(k)}$                      | Evaluate at $x=3$ |
| ------------------------------ | ----------------- |
| $x^{-1}$                       |                   |
| $-x^{-2}$                      |                   |
| $2x^{-3}$                      |                   |
| $-6x^{-4}$                     |                   |
| $f^{(k)} = (-1)^{k}k!x^{-k-1}$ | $(-1)^{k}$        |

$$\frac{1}{x}= \sum\limits_{k=0}^{\infty } \frac{(-1)^{k}k! 3^{-k-1 }}{k!}(x-3)^{k}$$
$$\frac{1}{x}= \sum\limits_{k=0}^{\infty} (-1)^{k}3^{-k-1} (x-3)^{k} = a_{k}$$

Ok, generally we need to find the IOC
So.... let's get to ratio testing

$$L = \lim\limits_{k \to \infty} \frac{(x-3)^{k+1} }{3^{k+2}}\cdot \frac{3^{k+1} }{(x-3)^{k}}$$
$$L = \lim\limits_{n \to \infty} \frac{(x-3)}{3}= \frac{|x-3|}{3}< 1$$
$$|x-3| < 3$$
$$-3 < x-3 < 3$$
$$0 < x < 6$$
So IOC is from 0 to 6, not including the endpoints $(0,6)$
we need to go test the endpoints separately to figure out what's going on

#### testing the endpoints

$$\sum\limits_{k=0}^{\infty} (-1)^{k}\frac{(0-3)^{k}}{3^{k+1} }$$
$$\sum\limits \frac{3^{k}}{3^{k+11}}$$
$$\sum\limits_{k=0}^{\infty} \frac{1}{3}$$
6 diverges by oscillation


-----------------


Find MacLauren series of $f(x) = \sin(x)$


| k   | $f^{(k)}$  | $f^{(k)}(0)$ |
| --- | ---------- | ------------ |
| 0   | $\sin(x)$  | 0            |
| 1   | $\cos(x)$  | +1           |
| 2   | $-\sin(x)$ | 0            |
| 3   | $-\cos(x)$ | -1           |
| 4   | $\sin(x)$  | 0            |
| k   |            |              |

$$\sin(x) = \sum\limits_{k=0}^{\infty} \frac{(-1)^{k}1}{(2k+1)!}x^{2k+1}$$
$$IOC = (-\infty,\infty)$$
$$ROC = \infty$$
What is the $f(x)$ for
$$\sum\limits_{k=0}^{\infty} \frac{(-1)^{k}1}{(2k+1)!}(3x)^{2k+1}$$
That's literally just $\sin(3x)$


----


Find T.S. of $\cos(x)$ centered at 0 
(MacLauren series)

$$\sin(x) = \sum\limits_{k=0}^{\infty} \frac{(-1)^{k}1}{(2k+1)! }x^{2k+1}$$
$$\frac{d}{dx}\sin(x) = \frac{d}{dx}\sum\limits_{k=0}^{\infty}(-1)^{k} \frac{1}{(2k+1)!}x^{2k}+1 $$
$$\cos(x) = \sum\limits_{k=0}^{\infty} (-1)^{k} \frac{1}{(2k+1)!} \frac{d}{dx}x^{2k+1}$$
$$\cos(x) = \sum\limits_{k=0}^{\infty} (-1)^{k} \frac{1}{(2k+1)!} (2k+1) x^{2k}$$
$$\sum\limits_{k=0}^{\infty} (-1)^{k} \frac{1}{(2k)!}x^{2k}$$
$$= 1 - \frac{x^{2}}{2!} + \frac{x^{4}}{4!}$$
Hey that's quirky, cos is even and sine is odd

$$ROC = \infty ~ => IOC = (-\infty,\infty)$$

---


We will have the taylor series for $e^{(x),}\sin(x), \cos(x), \frac{1}{1-x}, \ln(1+x)$


Applying TS

Approximate $$\int_{0}^{1} e^{-x^{2}}dx$$
to within 0.001 of its true value

$$e^{x} = \sum\limits_{k=0}^{\infty} \frac{x^{k}}{k! }$$

$$e^{-x^{2}}= \sum\limits_{k=0}^{\infty} \frac{(-x^{2})^{k}}{k!}$$
$$\sum\limits_{k=0}^{\infty} \frac{(-1)^{k}}{k!} x^{2k}$$
$$\int_{0}^{1}e^{-x^{2}}dx  = \sum\limits_{k=0}^{\infty} \frac{(-1)^{k}}{k!}x^{2k}dx$$
$$\sum\limits_{k=0}^{\infty } \frac{(-1)^{k}}{k!} \int_{0}^{1}x^{2k}dx$$
$$\sum\limits_{k=0}^{\infty} \frac{(-1)^{k}}{k!} \frac{x^{2k+1}}{2k+1}\Big|_{0}^{1}$$

$$[ x- \frac{x^{3}}{3} + \frac{x^{5}}{2!5} - \frac{x^{7}}{3!7}]$$
$$= 1 - \frac{1}{3}+ \frac{1}{10}- \frac{1}{42}$$
Use AST to show converge

$$| R_{k}| < | a_{k+1}|$$
$$a_{k}= \frac{1}{(k!)(2k+1)}< 0.001$$

