#notes #math112 #math #calc 


$$u = < 3,5,0>$$
$$v = <0,3,-6>$$
Find the projection of u onto v
$$\text{proj}_{v}(u)= c \cdot\vec{v}$$

$$\text{proj}_{v}(u) = \frac{\vec{u}\cdot\vec{v}}{|\vec{v}|^{2}}\vec{v}$$
$$\vec{u } \cdot \vec{v} = (0) + 15 +0$$
$$|v| = \sqrt{ 9 + 36} = \sqrt{45}^{2}= 45$$
$$\text{proj}_{v}(u)= \frac{15}{45}\vec{v} = \frac{1}{3}\vec{v}$$
$$\text{proj}_{v}(u) = <0, 1, -2>$$

---


$$\int \frac{x}{\sqrt{x-5}}dx$$

---

$$u = x-5, du = dx$$
$$\int \frac{x}{\sqrt{u}}du= \int \frac{u+5}{\sqrt{u}}du$$
$$\int \frac{u}{\sqrt{u}} + \frac{5}{\sqrt{u}}$$
$$\int \frac{u}{\sqrt{u}}+ 5\int \frac{1}{\sqrt{u}}$$
$$\int \frac{u}{\sqrt{u}}+ 5\int u^\frac{-1}{2}$$
$$\int \frac{u}{\sqrt{u}}+ 5 ( \frac{1}{2}u^\frac{1}{2})$$

---

$$\int u^\frac{1}{2}+ 5u^\frac{-1}{2}du$$
$$ \frac{u^{\frac{3}{2}}}{\frac{3}{2}} + 5 \frac{u^{\frac{1}{2}}}{\frac{1}{2}}+C$$
and y'know, plug u back in


---

$$\int (x) (x-5)^\frac{1}{2}dx$$




$$u = x$$
$$dv = (x-5)^{\frac{-1}{2}}dx$$



| u   | dv              |
| --- | --------------- |
| x   | $(x-5)^{-1/2}$  |
| dx  | $-2(x-5)^{1/2}$ |
| 0   | $3(x-5)^{3/2}$  |

$$(2x)(x-5)^{\frac{1}{2}} - \frac{4}{3}(x-5)^{\frac{3}{2}+}C$$
$$(2x)(x-5)^{\frac{1}{2}} - 3(x-5)^\frac{3}{2}$$


----


$$\sum\limits_{k=0}^{\infty} (-1)^{k}\frac{3^{2k}x^{2k}}{(2k)!}$$
$$\cos(x) = \sum\limits_{k=0}^{\infty} \frac{(-1)^{k}x^{2k}}{(2k)!}$$
$$\cos(3x) = \sum\limits_{k=0}^{\infty} \frac{(-1)^{k}(3x)^{2k}}{(2k!)}$$


---

$$\ln(1-x)= \sum\limits_{k=0}^{\infty} (-1)^{k+1} \frac{(-x)^{k}}{k}$$
$$\sum\limits_{k=1}^{\infty} \frac{(-1)^{k+1}(-1)^{k}x^{k}}{k}$$


-----


$$p1: x+y - z = 1$$
$$p2: 2x - 3y + 4z$$
There's a roundabout solving method, or

$$<1, 1, -1> \times <2, -3, 4>$$
$$<1,1,-1$$
$$<2,-3,4>$$
$$= < (4) - 3 , - (4 + 2), (-3 - 2) >$$
$$< 1, -6, -5>$$
Try something like $x=0$
$$y-z = 1$$
$$-3y + 4z = 5$$
$$y = 1+z$$
$$-3(1+z) + 4z = 5$$
$$-3 - 3z + 4z = 5$$
$$-3 + z = 5$$
$$ z= 8$$
$$y = 9$$
$$<0,9,8>$$
$$x = 0 + 1t$$
$$y = 9 - 6t$$
$$z = 8 -5t$$
