#notes #math112 #math #calc 

## previously on

$$\int_{0}^{1}e^{-x^{2} } = \int_{0}^{1}\sum\limits_{k=0}^{\infty} \frac{(-x^{2)^{k}} }{k!} = \sum\limits_{k=0}^{\infty} \frac{(-1)^{k}}{k!} \int_{0}^{1}x^{2k}dx $$
$$I = \sum\limits_{k=0}^{\infty} \frac{(-1)^{k}}{k!} \frac{x^{2k+1}}{2k+1}$$


----


$$P = (3,31)$$
$$Q = (2, -1, 0)$$
$$R = (-1, -3, 1)$$
$$Ax + By + Cz = D$$

$$PQ = (-1, -4, -1)$$
$$PR = (-4, -6, 0)$$
Cross product o those fellers, and you should end up with

---


$$x = 2 + s$$
$$y = 21 + 7s$$
$$z = 15 + 4s$$

bloop

$$x = -5 + 2t$$
$$y = -18 + 9t$$
$$z = -11 + 7t$$

----


one


Circle with radius $r=2$
Center at $(-1, 2)$
CCW


Ok, so if we have 

$$x = \cos(\theta)$$
and 
$$y = \sin(\theta)$$
that's just our unit circle, but let's do some modifications

$$ x= 2\cos(\theta), y = 2\sin(\theta)$$
that gets our radius of two
Aaaand then we just want to shift it over

$$x = 2\cos(\theta) - 1, y = 2\sin(\theta) + 2$$
$$\theta \epsilon [ 0,2\pi]$$


$$x = e^{t}+1$$
$$y = e^{3t}-2$$
$$x-1 = e^{t}$$
$$\ln(x-1) = t$$
$$y = e^{3\ln(x-1)}-2$$
$$y = e^{\ln(x-1)^{3}}-2$$
$$y = (x-1)^{3}-2 $$
