#notes #math112 #math #calc



Given that $$f(x) = \sum\limits c_{k}(x-a)^{k}$$
If the series converges for x= b, then it converges for all x such that $$| x-a| < | b| $$
where a is the center

If it diverges for $x=d,$ then it diverges for all $x$ such that $|(x-a) > |d|$

----


Time to start representing various $f(x)$ as power series

Start with some base series that we know, and then build off of it
	That base series is $$f(x) = \frac{1}{1-x} = \sum\limits_{k=0}^{\infty}x^{k} $$
Use algebra tools and calculus tools to build new power series

Given $f(x) = \sum\limits_{k=0}^{\infty} d_{k} x^{k}$
both w/ IOC = $I$

$$f(x) \pm g(x) = \sum\limits_{k=0}^{\infty} (c_{k}\pm d_{k})x^{k}$$
IOC = I

### multiply by $x^{m}$
m is an integer, and $m+k \geq 0$ for all $c_{k}\neq 0$

$$x^{m}f(x) = x^{m}\sum\limits_{k=0}^{\infty} c_{k}x^{k+m }$$
$$= \sum\limits c_{k}x^{k+m }$$
#### composistion
Let $h(x) = b x^{m}$
$f(h(x))$

$$\sum\limits_{k=0}^{\infty} c_{k}(h(x))^{k}$$
$$= \sum\limits_{k=0}^{\infty} c_{k}b^{k}x^{mk}$$
IOC: All x such that $h(x)$ is in $I$ (the original IOC)


----
$$f(x) = \frac{1}{{1+x^{4} }} = \frac{1}{1-(-x^{4})}$$
$$h(x) = (-1)x^{4}$$
Use composition
$$f(x) = \sum\limits_{k=0}^{\infty} = (-x^{4})^{k}$$
$$\sum\limits_{k=0}^{\infty} (-1)^{k}(x^{4k})$$
Find $| -x^{4}| < 1$
$$|x| < 1^\frac{1}{4}$$
$$IOC = (-1,1)$$



---


$$f(x) = \frac{x^{5}}{1+2x} $$
$$f(x) = x^{5} ~ * ~ \frac{1}{{1-(-2x)}}$$
$$h(x) = -2x$$

$$x^{5}\sum\limits_{k=0}^{\infty} (-2x)^{k}$$
$$= x^{5}\sum\limits _{k=0}^{\infty}(-2)^{k}x^{k}$$
$$\sum\limits -2^{k}x^{k+5}$$
$$IOC: |-2x| < 1  => 2 |x| < 1 = > |x| < \frac{1}{2}=> (\frac{-1}{2}, \frac{1}{2})$$

## the calculus tools
- Calculus
- Derivative
	- $$f(x) = \sum\limits_{k=0}^{\infty} c_{k}x^{k}= c_{0} + c_{1}x$$
	- $$f(x) = c_{0}+ c_{1}(x-a) + c_{2}(x-a)^{2}....$$
	- $$f'(x) = 0 + c_{1}+ c_{2}2(x-a) + c_{3}3(x-a)^{2}$$
	- $$f'(x) = \sum\limits_{k=1}^{\infty}c_{k}k (x-a)^{k-1}$$
	- With the same ROC = R
	- We could also reindex $\ell = k-1$ 
	- $$k = \ell + 1$$
	- $$\sum\limits_{\ell = 0}^{\infty}c_{\ell+1}(\ell+1)(x-a)^{\ell}$$

---

Example

Previously, we had $$f(x) = \sum\limits_{k=0}^{\infty} \frac{1}{k!} x^{k}$$
$$IOC = (-\infty, \infty)$$
$$f(x) = \frac{1}{0!} x^{0}+ \frac{1}{1!}x^{1}+ \frac{1}{2!}x^{2}$$
$$f'(x) = 0 + 1 + \frac{2}{2!}x + \frac{3}{3!} x^{2}+ ....$$
$$f'(x) = 1 + x + \frac{1}{2!}x^{2}+ \frac{1}{3!}x^{3} $$
$$f(x) = e^{x}$$