#notes #math112 #math #calc



$$\frac{x}{1-x}= x * \frac{1}{1-x}= x(1 + x + x^{2})$$


---


## just to reiterate

$$f(x) = \sum\limits_{k=0}^{\infty} \frac{f^{(k)}(a)}{k!}(x-a)^{k}$$
A is the center
Power series are unique
Find ioc


$$f(x) = e^{x}$$
$$f^{(0)}= e^{x}$$
$$f^{(1)}=e^{x}$$
and so on and so forth
Center at $x=0$, which is also a maclauren series
$$f^{(0)}(0) = 1$$
$$f^{(1) }(0) = 1$$
yadayadayadayadayada

$$= \sum\limits_{k=0}^{\infty} \frac{1}{k! }(x-0)^{k}$$
IOC for $e^{x}=(-\infty,\infty)$
We also might get something like approximate $e^{1}$ with five terms of the taylor series

$$e^{x}\approx 1 + x + \frac{x^{2}}{2!} + \frac{x^{3}}{3!}+ \frac{x^{4}}{4!} $$
Plugging in $x=1$
$$1 + 1 + \frac{1}{2}+ \frac{1}{6}+ \frac{1}{24}$$

----

Alright, we're still doing $e^{x}$, but now we're going to center at like, four

So they're all going to be e^4 

$$e^{x}= \sum\limits_{k=0}^{\infty} \frac{e^{4}(4)}{k!}(x-a)^{k}$$

---

#### Find IOC

Let $L =  \lim\limits_{k \to \infty}$

$$L = \lim\limits_{k \to \infty} \frac{e^{4}(x-4)^{k+1}}{(k+1)!} * \frac{k!}{e^{4}(x-4)^{k}}$$
$$\lim\limits_{n \to \infty} \frac{(x-4)}{k+1}$$
$$| (x-4)| \lim\limits_{k \to \infty} \frac{1}{k+1} =0<1$$

Use five terms to estimate $e^{1}$

$$e^{x}\approx e^{4}+ e^{4}(x-4) + \frac{e^{4}(x-4)^{2}}{2!}+ \frac{e^{4}(x-4)^{3}}{3!}+ \frac{e^{4}(x-4)^{4}}{4!} $$ 