#notes #math112 #math #calc 


##### converges absolutely or conditionally?

$$\sum\limits_{n=1}^{\infty} \frac{(-1)^{n}}{1+n^\frac{1}{2}}$$
AST says we converge, but conditional or absolute?

$$\sum\limits_{n=1}^{\infty} \frac{1}{1+n^\frac{1}{2}}$$


----
$$\int_{-1}^{1}e^{\frac{-x^{2}}{2}}$$

$$e^{x}= \sum\limits_{k=0}^{\infty} \frac{x^{k}}{k!} $$

$$e^{\frac{-x^{2}}{2}}= \sum\limits_{k=0}^{\infty} \frac{(\frac{-x^{2}}{2})^{k}}{k!} = \sum\limits_{k=0}^{\infty } \frac{(-1)^{k}(\frac{1}{2})^{k}x^{2k}}{k!}$$
$$\int_{-1}^{1 }e^{\frac{-x^{2}}{2}}dx = \int_{-1}^{1} \sum\limits_{k=0}^{\infty}(-1)^{k}a_{k}x^{2k}dx$$
$$\sum\limits_{k=0}^{\infty} \int_{-1}^{1}(-1)^{k}a_{k}x^{2k}$$
$$= \sum\limits_{k=0}^{\infty}(-1)^{k}a_{k}\int_{-1}^{1}x^{2k}= \sum\limits_{k=0}^{\infty}(-1)^{k}a_{k} \frac{x^{2k+1}}{2k+1}$$

$$\sum\limits_{k=0}^{\infty} (-1)^{k}a_{k} \frac{1}{2k+1} - \sum\limits_{k=0}^{\infty} (-1)^{k}a_{k}\frac{-1}{2k+1}$$
$$2\sum\limits_{k=0}^{\infty}(-1)^{k} a_{k} \frac{1}{2k+1} $$


$$2 \sum\limits_{k=0}^{\infty} (-1)^{k} \frac{(\frac{1}{2})^{k}}{k!} \cdot \frac{1}{2k+1}$$
$$ \text{Use alternating series remainder}$$
$$k_{5}= -0.000047, \text{so use first 5 terms (k=0 -> k=4 )}$$




----


### find t.s of $\sin(x)$ centered at $x=0$


$$\sin(x) = \sum\limits_{k=0}^{\infty} \frac{f^{(k)}(0)}{k!}(x-0)^{k}$$


| k   | $f^{k}(x)$ | $f^{k}(0)$ |
| --- | ---------- | ---------- |
| 0   | $\sin(x)$  | 0          |
| 1   | $\cos(x)$  | 1          |
| 2   | $-\sin(x)$ | 0          |
| 3   | $-\cos(x)$ | -1         |
| 4   | $\sin(x)$  | 0          |

$$\sin(x) = \frac{f^{(0)}(0)}{0!}x^{0}+ f^{(1)}\frac{0}{1!}x^{1}+ \frac{f^{(2)}(0)}{2!}x^{2}$$

$$= 0 + \frac{1}{1!}x^{1}+ 0 - \frac{1}{3!}x^{3}+ 0 ~ .......$$
$$= x - \frac{x^{3}}{6}+ ......$$
 