#notes #math112 #math #calc

Find $\Sigma$  notation for
$$s = 3e^{-1} + 3{e^{-2}} + 3^{-3}....$$
$$\sum\limits _{k=1}^{\infty} 3e^{-k}$$


$$S = \frac{1}{16}+ \frac{3}{64} + \frac{4}{256} + \frac{5}{1024}$$
$$\cancel{\sum\limits _{k=0}^{\infty} \frac{3^{k}}{2^{2k+2}}}$$
$$\sum\limits _{k=1}^{\infty} \frac{3^{k-1}}{2^{2k+2}}$$

$$s = \frac{-1}{2}+ \frac{4}{4}- \frac{9}{8}+ \frac{16}{16} - \frac{25}{32}$$
$$\sum\limits_{k=1}^{\infty} \frac{(-1)^{k}k^{2}}{2^{k}}$$

---



$$\sum\limits_{n=1} ^{\infty} \frac{1}{2+3^{n}}$$
At extrema, this is basically$$\frac{1}{3^{n}}, = 3^{-n}$$

so using direct comparison
Which is a geometric series with $r < 1$, so converges

$$\sum\limits_{n=1}^{\infty} \frac{2^{n}}{n^{3} }$$
$$\lim\limits_{n \to \infty} \frac{2^{n}}{n^{3}}= \infty, \text{diverges by divergence test}$$
$$\text{(with growth rates)}$$

----



$$\sum\limits_{n=1}^{\infty} \frac{1}{{(n^{2}+2n)}^{\frac{1}{3}}}$$
