#notes #math112 #math #calc




## root test

- Given $\sum\limits a_{k}$, let $\rho = \lim\limits_{n \to \infty} |a_{k}|^{1/k}$ 
	- If $\rho < 1,$ then $\sum\limits a_{k}$ converges absolutely
	- If $\rho > 1$, then $\sum\limits a_{k}$ diverges
	- If $\rho =1$, then we're inconclusive

#### example
$$\sum\limits_{k=1} ^{\infty} \left(\frac{3}{4}\right)^{k}$$
$$\rho = \lim\limits_{n \to \infty}\left( \left( \frac{3}{4}\right)^{k}\right)^{\frac{1}{k}}$$
$$\rho = \lim\limits_{n \to \infty} \frac{3}{4}= \frac{3}{4}$$
Which is less than one, so that sure looks like it converges absolutely

#### trickier example
$$\sum\limits _{k=1}^{\infty} ( 1 + \frac{2}{k})^{k^{2} } $$
Power depends on k, so good canidate to get rooty with it

$$\rho = \lim\limits_{n \to \infty} \left(\left( 1+ \frac{2}{k}\right)^{k^{2}}\right)^{\frac{1}{k}}$$
$$\lim\limits_{n \to \infty} ( 1+ \frac{2}{k})^{k}= 1^{\infty}$$
That's a problem
$$\ln\rho = \lim\limits_{n \to \infty}\ln\left(\left( 1 + \frac{2}{k}\right)^{k}\right) $$
$$\ln(\rho) = \lim\limits_{n \to \infty} k \ln(1 + \frac{2}{k})= \infty * 0$$
That's a problem, again

$$\ln\rho = \lim\limits_{n \to \infty} \frac{\ln(1 + \frac{2}{k})}{\frac{1}{k}}= \frac{0}{0}$$
That's a problem again 

$$ \frac{\frac{1}{1+ \frac{2}{k}}* \frac{-2}{k^{2}}}{\frac{-1}{k^{2}}}$$
$$\frac{\frac{-2}{1}}{-1}$$
$$\ln(\rho) = 2$$
$$\rho = e^{2}$$
P-like series are absolutely going to come out to be one


----

$$\int \frac{\sqrt{9-x^{2}}}{x}dx$$
$$x = 3\sin(\theta)$$

You can get a triangle, hypotenuse is three,you end up with $\sqrt{9-x^2}$ for the missing side

$$dx = 3\cos(\theta)d\theta$$
$$\int \frac{\sqrt{9 - 9\sin^{2}\theta}}{3\sin(\theta)}(3\cos(\theta)d\theta)$$
$$\int 3 \frac{\cos\theta}{\sin(\theta)}3\cos\theta d\theta $$
$$\int \cos^{2}\theta * (\sin(\theta))^{-1} d \theta$$
$$3 \int \cos^{2}\theta ( \sin\theta)^{-2} \sin(\theta)d\theta$$
$$u = \cos\theta, du = -\sin\theta d\theta$$
$$3 \int u^{2}\frac{1}{1-u^{2} }(-du)$$
$$3 \int \frac{u^{2}}{u^{2}-1}du$$
$$\int 1 + \frac{1}{u^{2}-1} $$
$$\int ( 1 + \frac{1}{(u+1)(u-1)})du$$
$$ \frac{A}{u+1} +  \frac{B}{u-1} $$
$$A = \frac{1}{2}, B = \frac{-1}{2} $$
$$I = $$
ooooooor, less annoying way

$$3 \int ( 1 - \sin^{2}\theta) \frac{1}{\sin\theta}d\theta $$
$$3 \int (\frac{1}{\sin\theta} - \sin\theta)d\theta$$
$$3 \int ( \csc\theta - \sin\theta)d\theta$$



----

$$\int \frac{z^{2}}{(z^{2}+ 36)^{2}}$$
$$z = 6\tan(\theta)$$

$$\int  \frac{36\tan^{2}\theta}{(36\tan^{2}\theta + 36)^{2}}(6 \sec^{2}\theta d\theta)$$
$$( 36(\tan^{2}\theta) + 1))^{2}
$$$$\int \frac{36\tan^{2}\theta}{(36 \sec^{2}\theta)^{2}}$$
$$\frac{36*6}{36^{2}}  \int \frac{\tan^{2}\theta \sec^{2}\theta}{\sec^{4}\theta}d\theta$$
$$\frac{1}{6}\int \frac{\sin^{2}\theta}{\cos^{2}\theta} * \cos^{2}\theta= \frac{1}{6}\int \sin^{2}\theta$$
$$\frac{1}{6}\int \frac{1-\cos(2\theta)}{2}= $$









---


$$\int \frac{dx}{\sqrt{x^{2}- 81}}$$
$$x = 9\sec(\theta)$$


----




$$ I = \int \frac{16x^{2} }{(x-6)(x+2)^{2} }$$
$$= \frac{A}{x-6} +  \frac{B}{x+2} + \frac{C}{(x+2)^{2}} $$


----

$$\int \frac{8(x^{2}+4)}{x(x^{2}+8)}dx$$
$$= \frac{A}{x}+ \frac{Bx+c}{x^{2}+8}$$
Coverup gives $$ A = \frac{16x^{2}}{(x+2)^{2}}= \frac{16*36}{64} =9 $$
$$C = \frac{16x^{2}}{x-6}= \frac{16(4)}{(-8)}=-8$$
For b, just plug something in for x

$$ 0 = \frac{9}{-6} + \frac{B}{2}  + \frac{-8}{4}$$
$$B = 7$$

---


$$\int _{1}^{2} \frac{dx}{\sqrt{x-1}}$$
Replace the integral, and then let $n$ go to 1 from the right

---

$$\int _{1}^{\infty} \frac{dx}{x^{2}(x+1)}$$
$$\int_{a}^{b} \frac{dx}{x^{@(x+1)}} $$
Let a go to 1, let b go to infty
