#notes #math112 #math #calc

We have some geometric series as k goes to infinity of $ar^{k}$ 
- Which converges upon some value $\frac{a}{1-r}$ if $|r|<1$ 
- For literally any other situation it diverges


$$\sum\limits _{k=3}^{\infty}3 ( \frac{3}{4})^{k}$$


$$\text{Let } l = k-3 $$
Which sets 
$$k= l+3$$
$$s = \sum\limits _{l=0}^{\infty} 3(\frac{3}{4})^{l+3}$$
Works as $$3*\left(\left(\frac{3}{4}\right)^{l}* (\frac{3}{4})^{3}\right)$$
$$a = \frac{81}{64}, r= \frac{3}{4}$$
$$\sum\limits _{l=0}^{\infty} \frac{81}{64}( \frac{3}{4})^{l}$$
$$S = \frac{\frac{81}{64}}{\frac{1}{4}}$$
$$S = \frac{81}{64}*4 = \frac{81}{16}$$
Alternatively, 


$$s = \sum\limits _{k=0}^{\infty} 3(\frac{3}{4})^{k} - \text{all the terms from 0 to 2}$$
When $k=1$, it just ends up being $$\frac{ar}{r-1} $$

---


## telescoping series
$$s = \sum\limits_{k=1}^{\infty}( \cos(\frac{1}{k})-\cos(\frac{1}{{k+1}}))$$


So the partial sum at any given point is just $$\cos(1)-\cos(\frac{1}{n+1})$$

So our limit is just $$\cos(1)-\cos(0), \text{or} \cos(1)-1$$


---


$$s = \sum\limits_{k=1}^{\infty} \frac{1}{k(k+1)}$$