#notes #math112 #math #calc

- If you're in a situation where you have a transcendental \* a transcendental, pretty good odds you end up in some cyclical bullshit


- Exam statistics
	- Median of 72, maxium of 97, mean of 73.25, Standard Deviation of 14.36

$$\int 12 \cos^{4}(3x)dx$$
$$12\int \cos^{2}(3x)\cos^2(3x)$$
$$12 \int \frac{1+\cos(6x)}{2}*\frac{1+\cos(6x)}{2}$$
$$12 \int \frac{1+2\cos(6x)+\cos^{2}(6x)}{4}$$
$$3\int 1+2\cos(6x)+\cos^{2}(6x)$$
$$12\int \frac{1+2\cos(6x)+\cos^2(6x)}{4}$$
$$3\int 1 + 2\cos(6x) + \frac{1+\cos(12x)}{2}$$

---

In a situation where you end up with irreducible quadratic factors 
 (ie, $x^{2}+1$) has no real roots
- For irreducible $x^{2}+bx+c$, 

$$\frac{Ax+b}{x^{2}+bx+c}$$


---


$$I = \int \frac{3x^{2}-4x+5}{(x-1)(x^{2}+1)}dx$$
- this is proper, we sure cannot factor the base
-

$$\frac{A}{x-1}+\frac{Bx+c}{x^{2}+1}dx$$
$$A = \frac{3x^{2}-4x+5}{x^{2}+1}$$
$$A = \frac{3-4+5}{1+1}=2$$
- for B and C we're..... gonna need to do more work

$$\frac{3x^{2}-4x+5}{(x-1)(x^{2}+1)}= \frac{2}{x-1} + \frac{Bx+c}{x^{2}+1}$$
Let x = 0, because that lets us find C by killing B (naur)

$$\frac{0-0+5}{-1(1)}= \frac{2}{-1}+ \frac{C}{1}$$
$$-5 +2 = C$$
$$C = -3$$

$$\frac{3x^{2}-4x+5}{(x-1)(x^{2}+1)}= \frac{2}{x-1}+ \frac{-3x+C}{x^{2}+1}$$
Let $x$ = $-1$

$$\frac{3+4+5}{(-2)(2)}=\frac{12}{-4}=-1$$
look, don't question it, you actually set it equal to the other sdie



-----



Repeated irreducible Quadratics

$$\int \frac{dx}{x(x^{2}+1)^{3}}= \int \frac{A}{x}+\frac{B_{1}x+C_{1}}{x^{2}+1}+ \frac{B_{2}x+C_{2}}{(x^{2}+1)^{2}}+ \frac{B_{3}x+C_{3}}{(x^{2}+1)^{3}}$$

---


### worksheet 2.7 \# 2


$$\frac{1}{x^{4}-1} = \frac{1}{(x^{2}+1)(x^{2}-1)} = \frac{1}{(x^{2}+1)(x+1)(x-1)}$$
$$\frac{A}{(x+1)}+ \frac{B}{(x-1)} + \frac{Cx+d}{(x^2+1)}$$


------------



## Briggs 8.9 - Improper integrals

##### type 1
- Happen when at least one end of the limit of integration is unbounded



$$\int _{0}^{\infty}e^{-2x}dx$$
The function is getting rather close to 0, as we go towards infinity

##### type 2
- happens when the integrand is unbounded

$$\int _{0}^{1} \frac{1}{x}dx $$
- that's fine, as it goes past 1

FTOC

$$\int _{a}^{b}f(x)dx = F(b)-F(a)$$
- where F is the antiderivative of $f$
- that's wonderful. toss that shit out. does not apply to improper integrals



##### type 1 (but again)
$$\text{Definition } \int _{a}^{\infty}f(x)dx = \lim\limits_{n \to \infty}\int _{a}^{n}f(x)dx$$
- Hey, if we use $n$ as a finite upper limit, we can evaluate *that* using the FTOC
	- so yeah, do that, evaluate with FTOC
- aaand then take the limit
- we kinda need $f(x)$ to be continuous on $x \geq a$, just as a note
- If the limit exists (spits a number out)
	- theeen, the improper integral converges on some value 
- If the limit does *not* exist
	- then the improper integral diverges

##### example
$$\int_{0}^{\infty}e^{-2x}dx = \lim\limits_{n \to \infty}\int_{0}^{n}e^{-2x}dx = \lim\limits_{n \to \infty} \frac{-1}{2}e^{-2x}|_{0}^{n} $$
$$= \lim\limits_{n \to \infty}( -\frac{1}{2}e^{-2n}+ \frac{1}{2}e^{0}) $$
$$= \lim\limits_{x \to y} ( - \frac{1}{2}* \frac{1}{e^{2n}} + \frac{1}{2})$$
$$= \frac{1}{2}$$
##### example 2
$$\int _{1}^{\infty} \frac{1}{x}dx$$
$$= \lim\limits_{n \to \infty} \int _{1}^{n} \frac{1}{x}dx = \lim\limits_{n \to \infty} \ln(x) |_{1}^{n}$$
$$= \lim\limits_{n \to \infty}\ln(n)=\infty$$

