#notes #math112 #math #calc

- Linear approximation
	- Given $f(x)=e^{1-x}$
	- Approximate this with a linear function centered at $x=1$
		- SO the slope, $f'(x)= -e^{1-x}$
		- $f'(1)=-e^{0}=-1$
		- 
- Quadratic Approximation
- Polynomial Approximation
	- Taylor polynomials
- 
point
$$(1,f(1)) = (1,1)$$
$$y - f(1) = f'(1)(x-1)$$
$$L(x) = 2-x \approx e^{1-x}$$
Most accurate for $x$ near 1

Lettuce approximate $e^\frac{1}{4}$
Evaluate L at $\frac{3}{4}$, so then we get L = $\frac{5}{4}$, which has an error of $0.034025$

----


Now we're up to
#### quadratic approximation
( we're generally going to $x^{n},$ eventually to approximate at $x=a$

$$P_{0}(x) = f(a)$$
$$P_{1}(x) = f(a) + f'(a)(x-a)$$
$$P_{2}(x) = f(a) + f'(a)(x-a) + \frac{f''(a)}{2}(x-a)^{2}$$
$$P_{2}(a) = f(a) + 0 + 0$$
$$P''_{2}(x) = \frac{f''(a)2}{2}= f''(a)$$

---

|                    |            |
| ------------------ | ---------- |
| $f(x) = e^{1-x}$   | $f(1)=1$   |
| $f'(x) = -e^{1-x}$ | $f'(1)=-1$ |
| $f''(x)=e^{1-x}$   | $f''(1)=1$ |
$$P_{2}(x) = 1 + (-1)(x-1) + \frac{1}{2}(x-1)^{2}$$
$$P_{2}(x) = \frac{5}{2}- 2x + \frac{1}{2}x^{2}$$
$$e^{\frac{1}{4}=\frac{}5}{2}- 2\left(\frac{3}{4}\right)+ \frac{1}{2}\left(\frac{3}{4 }\right)^{2}$$


### Taylor Polynomials
Given $f(x)$ with derivatives
- these are all going to be things that we can keep taking derivatives of
	- $f'(x) = f^{1}(x)$ 
	- We're going to keep using power notation, because we're throwing a lot of primes on
	- Base function is $f^{(0)}(x)$
	- $0!=1$ lol, bozo, L, does that shit make sense? no. eat shit.
- Polynomial centered at $x=a$
- $P_{n}(x) = f(a) + f^{(1)}(a)(x-a)+ f^{(2)}\frac{a}{2!}(x-a)^{2}+ .... \frac{f^{(n)(a)}}{n!}(x-a)^{n}$ 

$$P_{n}(x) = \sum\limits _{k=0}^{n} \frac{f^{(k)}(a)}{k!}(x-a)^{k}$$

---



| $f^{(0)}=\cos(x)$  | $f(\pi/2)=0$    |
| ------------------ | --------------- |
| $f^{(1)}=-\sin(x)$ | $f'(\pi/2)=-1$  |
| $f^{(2)}=-\cos(x)$ | $f''(\pi/2)=0$  |
| $f^{(3)}=\sin(x)$  | $f'''(\pi/2)=1$ |
|                    |                 |
$$P_{3}=f\frac{\pi}{2}+ f'\left(\frac{\pi}{2}\right)\left( x - \frac{\pi}{2}\right)+ f''\frac{\frac{\pi}{2}}{2!}(\frac{x-\pi}{2})^{2} + \frac{f'''(\pi/2)}{3!}(x-\pi/2)^{3}$$
$$P_{3}= -1 (x-\pi/2)+1/6(x-\pi/2)^{3}$$
