#notes #math112 #math #calc



Last time, we had our starting series $$f(x) = \frac{1}{1-x} = \sum\limits_{k=0}^{\infty}x^{k}$$
Which had an IOC of $$(-1, 1)$$
Derivative Tool

$$f(x) = \sum\limits_{k=0}^{\infty}c_{k}(x-a)^{k}$$
We went on and derived that, and got
$$f'(x) = \sum\limits_{k=1}^{\infty} c_{k}k (x-a)^{k-1}$$


----


### example (similar to worksheet)
Find the power series of $g(x) = \frac{1}{(1-x)^{2}}$

$$f'(x) = \frac{d}{dx}\left(\frac{1}{1-x}\right)= \frac{d}{dx}(1-x)^{-1} = - (1-x)^{-2}= \frac{-1}{(1-x)^{2}}$$
$$g(x) = - f'(x)$$
$$g(x) = - \frac{d}{dx}\sum\limits_{k=0}^{\infty}$$
$$g(x) = - \sum\limits_{k=1}^{\infty} kx^{k-1}$$
$$f(x), ROC = 1$$
$$ROC \text{ is in fact, still 1}$$

----

### Integration

$$f(x) = \sum\limits_{k=0}^{\infty} c_{k}(x-a)^{k}$$
$$\int f(x)dx = \int \sum\limits_{k=0}^{\infty} c_{k}(x-a)^{k}$$
$$\int f(x) dx = \sum\limits_{k=0}^{\infty} c_{k}\int (x-a)^{k}dx$$
$$c_{0}\int (1) + c_{1}\int(x-a) + c_{2}\int(x-a)^{2}$$
$$c_{0}x + \frac{c_{1}(x-a)^{2}}{2} + \frac{c_{2}(x-a)^{3}}{3}....... + C$$
$$ = c_{0}x - c_{0}a + c_{0}a$$
Toss that $c_{0}a$ in the constant

$$= \sum\limits_{k=0}^{\infty} \frac{c_{k}(x-a)^{k+1}}{k+1} $$
ROC still.... doesn't change!

### example
Find the power series of $$g(x)= \frac{1}{1+x}$$
$$g(x) = \frac{1}{1-(-x)}$$
$$h(x) = -x$$
$$\sum\limits_{k=0}^{\infty} (-x)^{k}$$
$$\sum\limits_{k=0}^{\infty} (-1)^{k}x^{k}$$
$$\int \frac{1}{1+x}dx = \ln(1+x) + C$$
$$\int \sum\limits_{k=0}^{\infty} (-1)^{k}x^{k}dx = \sum\limits_{k=0}^{\infty} (-1)^{k}\frac{x^{k+1}}{k+1} +C$$
Usually we "lock teh constant"

$$\ln(1+0) = \sum\limits_{k=0}^{\infty} (-1)^{k} \frac{0^{k+1}}{k+1} +C$$
$$C = 0$$
$$\ln(1+x) = \sum\limits_{k=0}^{\infty} (-1)^{k}\frac{x^{k+1}}{k+1}$$
$$= x - \frac{x^{2}}{2}+ \frac{x^{3}}{3}- \frac{x^{4}}{4}........$$
Let's go test an endpoint, for shits and gigs

$x=1$
$$\ln(1+1)=\sum\limits _{k=0}^{\infty} \frac{(-1)^{k}1}{k+1} $$

---

$$g(x) = \tan^{-1}(x)$$
$$g'(x) = \frac{d}{dx}\tan^{-1}(x) = \frac{1}{1+x^{2}}$$
$$g'(x)= \frac{1}{1-(-x^{2})}$$
$$\sum\limits_{k=0}^{\infty} (-x^{2})^{k}$$
$$\sum\limits_{k=0}^{\infty}(-1)^{k}(x^{2})^{k}$$
$$\sum\limits_{k=0}^{\infty}(-1)^{k}x^{2k}$$
$$\tan^{-1}(x) = \sum\limits_{k=0}^{\infty}(-1)^{k} \frac{x^{2k+1}}{2k+1} +C$$
lockdown constant

$$\tan^{-1}(0) = 0 = 0 + C$$
$$\tan^{-1}(1)= \frac{\pi}{4}= 1 - \frac{1}{3}+ \frac{1}{5}- \frac{1}{7}$$


----


### Taylor Series

Theorem: If $f(x)$ has a power series representation, then 
$$f(x) = \sum\limits_{k=0}^{\infty} f^{(k)}\frac{a}{k!} (x-a)^{k}$$
- unique
- When $a=0$, it is also called a MacLauren series
- 